Added definitions for structural equivalence, merge, an equality that disregards first direction, lexicographical induction; put contracted definitions and lemmas into separate file; progress on cut elimination.

cut.v
@@ -10,842 +10,13 @@ Require Import lnt_weakeningT.
 Require Import lnt_contractionT.
 Require Import existsT.
 Require Import lnt_weakeningT lnt_contraction_mrT.
+Require Import ind_lex.
+Require Import contractedT.
+Require Import structural_equivalence.
+Require Import merge.
 
 
-(* TACTICS *)
 
-
-Ltac clear_useless :=
-  repeat match goal with
-         | [H : ?a = ?a |- _] => clear H
-         | [H : [?a] = [?a] |- _] => clear H
-         | [H : ?a :: ?b = ?a :: ?b |- _] => clear H
-         | [H1 : ?a, H2 : ?a |- _] => clear H2
-         end.
-
-Ltac inv_singleton :=
-    repeat ( match goal with
-       | [ H : ?a :: [] = ?c :: ?d |- _ ] => inversion H; subst
-       | [ H : ?a :: ?b = ?c :: [] |- _ ] => inversion H; subst
-(*        | [ H : ?a :: [] = ?c :: [] |- _ ] => inversion H; subst *)
-       | [ H : ?a :: ?b = ?c :: ?d |- _ ] => inversion H; subst
-(*           | [ H : ?b :: ?c = [?a] |- _ ] => inversion H; subst
-           | [ H : [?a] = ?b :: ?c |- _ ] => inversion H; subst
-           | [ H : ?b :: ?c = [?a] |- _ ] => inversion H; subst
-           | [ H : [?a] = [?b] |- _ ] => inversion H; subst
-           | [ H : [?b] = [?a] |- _ ] => inversion H; subst
-*)
-           | [ H : ((?a,?b) = ?c) |- _ ] => inversion H; subst
-           | [ H : ?c = (?a,?b) |- _ ] => inversion H; subst
-                           end; clear_useless).
-
-Ltac inversion_cons :=
-  repeat match goal with
-         | [ H : ?a :: ?l1 = ?b :: ?l2 |- _] => inversion H; subst; clear_useless
-         end.
-
-(* ------------------------- *)
-
-(* STRUCTURAL EQUIVALENCE *)
-                    
-(* Use this one to help with full structural equivalence definition. *)
-Inductive struct_equiv_str {V : Set} : (list (rel (list (PropF V)) * dir)) -> (list (rel (list (PropF V)) * dir)) -> Type :=
-| se_nil2 : struct_equiv_str [] []
-| se_step2 Γ1 Δ1 d Γ2 Δ2 ns1 ns2 ns3 ns4 :
-    ns3 = ((Γ1, Δ1, d) :: ns1) ->
-    ns4 = ((Γ2, Δ2, d) :: ns2) ->
-    struct_equiv_str ns1 ns2 ->
-    struct_equiv_str ns3 ns4.
-
-(* Use this one for structural equivalence. *)
-Inductive struct_equiv_weak {V : Set} : (list (rel (list (PropF V)) * dir)) -> (list (rel (list (PropF V)) * dir)) -> Type :=
-| se_wk2_extL ns1 ns2 ns3 ns4 :
-    ns4 = (ns1 ++ ns3) -> struct_equiv_str ns1 ns2 -> struct_equiv_weak ns4 ns2
-| se_wk2_extR ns1 ns2 ns3 ns4 :
-    ns4 = (ns2 ++ ns3) -> struct_equiv_str ns1 ns2 -> struct_equiv_weak ns1 ns4.
-
-Inductive struct_equiv {V : Set} n1 n2 : Type :=
-| se : @struct_equiv_weak V n1 n2 -> struct_equiv n1 n2.
-
-Lemma struct_equiv_str_weak : forall {V : Set} G1 G2,
-   @struct_equiv_str V G1 G2 -> @struct_equiv_weak V G1 G2.
-Proof.
-  intros V G1 G2 H.
-  eapply se_wk2_extL in H. 2 : reflexivity.
-  erewrite app_nil_r in H.  exact H.
-Qed.
-
-Lemma struct_equiv_str_length : forall {V : Set} G1 G2,
-    @struct_equiv_str V G1 G2 -> length G1 = length G2.
-Proof.
-  induction G1; intros H2 H; destruct H2;
-    subst; (reflexivity || inversion H).
-  discriminate. discriminate. 
-  subst. simpl. erewrite IHG1. reflexivity.
-  inversion H1. inversion H0. subst.
-  assumption.
-Qed.
-
-Lemma struct_equiv_weak_str : forall {V : Set} G1 G2,
-    @struct_equiv_weak V G1 G2 -> length G1 = length G2 ->
-    @struct_equiv_str V G1 G2.
-Proof.
-  intros V G1 G2 H1 H2.
-  inversion H1; subst;
-    rewrite app_length in H2.
-  inversion H0; subst. simpl in *.
-  apply length_zero_iff_nil in H2. subst.
-  constructor.
-  simpl; pose proof H4 as H4';
-  eapply struct_equiv_str_length in H4;
-  simpl in H2; rewrite H4 in H2;
-  destruct ns3; simpl in *; [
-  rewrite app_nil_r;  econstructor; try reflexivity; try assumption |
-  firstorder ].
-
-  inversion H0; subst. simpl in *.
-  symmetry in H2.
-  apply length_zero_iff_nil in H2. subst.
-  constructor.
-  simpl; pose proof H4 as H4';
-  eapply struct_equiv_str_length in H4;
-  simpl in H2; rewrite H4 in H2;
-  destruct ns3; simpl in *; [
-  rewrite app_nil_r;  econstructor; try reflexivity; try assumption |
-  firstorder ].
-Qed.
-
-Lemma struct_equiv_weak_cons : forall {V : Set} l1 l2 a1 a2,
-    struct_equiv_weak (a1::l1) (a2::l2) ->
-    @struct_equiv_weak V l1 l2.
-Proof.
-  intros V l1 l2 a1 a2 H3.
-  inversion H3 as [l3 H4 l4 H5 H6 H7 | H4 l3 l4 H5 H6 H7]; subst.
-  destruct l3 as [| a ns1];
-    inversion H7; try discriminate; subst.
-  simpl in *. unfold rel in *.
-  inversion_cons.
-  econstructor. reflexivity. assumption.
-
-  destruct l3 as [| a ns1];
-    inversion H7; try discriminate; subst.
-  simpl in *. unfold rel in *.
-  inversion_cons.
-  econstructor 2. reflexivity. assumption.
-Qed.
-
-Lemma struct_equiv_weak_cons_rev : forall {V : Set} l1 l2 a1 a2 b1 b2 d,
-    @struct_equiv_weak V l1 l2 ->
-    struct_equiv_weak ((a1,b1,d)::l1) ((a2,b2,d)::l2).
-Proof.
-  intros V l1 l2 a1 a2 b1 b2 d H3.
-  inversion H3; subst.
-  econstructor.
-  rewrite cons_singleton. rewrite app_assoc.
-  reflexivity.
-  econstructor 2; try reflexivity. assumption.
-
-  econstructor 2.  rewrite cons_singleton. rewrite app_assoc.
-  reflexivity.
-  econstructor 2; try reflexivity. assumption.
-Qed.
-
-Ltac struct_equiv_str_nil :=
-  match goal with
-  | [H : struct_equiv_str [] ?n |- _] => inversion H; discriminate
-  | [H : struct_equiv_str ?n [] |- _] => inversion H; discriminate
-  end.
-
-Ltac struct_equiv_str_cons :=
-  match goal with
-  | [H : struct_equiv_str (?a :: ?la) (?b :: ?lb) |- _] => inversion H; subst
-  end.
-
-Lemma struct_equiv_weak_d : forall {V : Set} ns1 ns2 seq1 seq2 d1 d2,
-    @struct_equiv_weak V ((seq1,d1)::ns1) ((seq2,d2)::ns2) ->
-    d1 = d2.
-Proof.
-  intros until 0; intros H3.
-  inversion H3 as [l3 H4 l4 H5 H6 H7 | H4 l3 l4 H5 H6 H7]; subst. 
-  destruct l3. simpl in *.
-  struct_equiv_str_nil.
-  simpl in *.
-  inversion_cons.
-  struct_equiv_str_cons. 
-  unfold rel in *. inversion_cons.
-  reflexivity.
-  
-  destruct l3. simpl in *.
-  struct_equiv_str_nil.
-  simpl in *.
-  inversion_cons.
-  struct_equiv_str_cons. 
-  unfold rel in *. inversion_cons.
-  reflexivity.
-Qed.  
-
-Lemma struct_equiv_str_weak_equiv : forall {V : Set} G1 G2,
-    iffT (@struct_equiv_str V G1 G2)
-         (struct_equiv_weak G1 G2 * (length G1 = length G2)).
-Proof.
-  intros.
-  split; intros HH. split. apply struct_equiv_str_weak.
-  assumption. apply struct_equiv_str_length. assumption.
-  apply struct_equiv_weak_str; apply HH.
-Qed.
-
-Lemma struct_equiv_weak_nil : forall (V : Set),
-    @struct_equiv_weak V nil nil.
-Proof.
-  econstructor. erewrite app_nil_r.
-  reflexivity. econstructor.
-Qed.
-  
-Lemma struct_equiv_str_refl : forall {V : Set} G, @struct_equiv_str V G G.
-Proof.
-  induction G as [|a G IHG]. constructor.
-  destruct a as [ [Γ Δ] d].
-  econstructor 2. reflexivity.
-  reflexivity. assumption.
-Qed.
-
-Lemma struct_equiv_weak_refl : forall {V : Set} G,
-    @struct_equiv_weak V G G.
-Proof.
-  intros V G. econstructor.
-  erewrite app_nil_r. reflexivity.
-  apply struct_equiv_str_refl.
-Qed.
-
-
-(* --------------------------- *)
-
-(* MERGE *)
-
-Inductive merge {V : Set} :  (list (rel (list (PropF V)) * dir)) ->  (list (rel (list (PropF V)) * dir)) ->  (list (rel (list (PropF V)) * dir)) -> Type :=
-| merge_nilL ns1 ns2 ns3 : ns1 = [] -> ns3 = ns2 -> merge ns1 ns2 ns3
-| merge_nilR ns1 ns2 ns3 : ns2 = [] -> ns3 = ns1 -> merge ns1 ns2 ns3
-| merge_step Γ Δ Σ Π d ns1 ns2 ns3 ns4 ns5 ns6 seq1 seq2 seq3 :
-    seq1 = (Γ,Δ,d) -> seq2 = (Σ,Π,d) -> seq3 = (Γ++Σ,Δ++Π,d) ->
-    merge ns1 ns2 ns3 ->
-    ns4 = seq1 :: ns1 -> ns5 = seq2 :: ns2 -> ns6 = seq3 :: ns3 ->
-    merge ns4 ns5 ns6.
-
-Lemma merge_existence {V : Set} : forall n1 n2,
-      struct_equiv_weak n1 n2 ->
-      existsT2 n3, @merge V n1 n2 n3.
-Proof.
-  induction n1; intros n2  Hequiv.
-  inversion Hequiv. subst. inversion H0; subst.
-  simpl in *. subst. exists nil. econstructor; reflexivity.
-  discriminate.
-  subst. inversion H0. subst. simpl in *.
-  exists ns3. econstructor 1; reflexivity.
-  discriminate.
-
-  destruct n2. exists (a :: n1). econstructor 2; reflexivity.
-  destruct a as [ [Γ1 Δ1] d1].
-  destruct p as [ [Γ2 Δ2] d2].
-  pose proof (struct_equiv_weak_d _ _ _ _ _ _ Hequiv). subst.
-  eapply struct_equiv_weak_cons in Hequiv.
-  eapply IHn1 in Hequiv. destruct Hequiv as [n3 Hn3].
-  exists ((Γ1 ++ Γ2, Δ1 ++ Δ2, d2) :: n3).
-  econstructor 3; try reflexivity. assumption.
-Qed.
-
-Lemma merge_consL : forall {V : Set} l l2 a b c,
-    @merge V (a :: l) [b] (c :: l2) ->
-    l = l2.
-Proof.
-  intros until 0; intros Hm.
-  inversion Hm; try discriminate;
-    inv_singleton; try reflexivity.
-  inversion X; try discriminate;
-  subst; reflexivity.
-Qed.  
-
-
-Lemma merge_consR : forall {V : Set} l l2 a b c,
-    @merge V [b] (a :: l) (c :: l2) ->
-    l = l2.
-Proof.
-  intros until 0; intros Hm.
-  inversion Hm; try discriminate;
-    inv_singleton; try reflexivity.
-  inversion X; try discriminate;
-  subst; reflexivity.
-Qed.  
-
-Lemma merge_unique {V : Set} : forall n1 n2 n3 n4,
-    struct_equiv_weak n1 n2 ->
-    merge n1 n2 n3 -> @merge V n1 n2 n4 -> n3 = n4.
-Proof.
-  induction n1; intros n2 n3 n4 Hs Hm1 Hm2.
-  inversion Hm1; subst; inversion Hm2; subst;
-    try reflexivity; try discriminate.
-
-  inversion Hm1; inversion Hm2; subst; try discriminate; try reflexivity;
-    inv_singleton; try reflexivity.
-
-  all : try solve [inversion X; subst; try reflexivity; try discriminate].
-
-  eapply IHn1 in X; [ | | exact X0].
-  subst. reflexivity.
-  eapply struct_equiv_weak_cons. exact Hs.
-Qed.
-
-Lemma merge_struct_equiv_weak : forall {V : Set} G1 G2 G3,
-  merge G1 G2 G3 ->
-  @struct_equiv_weak V G1 G2.
-Proof.
-  induction G1; intros G2 G3 H.
-  + inversion H; try discriminate.
-    econstructor 2. erewrite app_nil_l. reflexivity. econstructor.
-    econstructor 2. erewrite app_nil_l. reflexivity. econstructor.    
-  + inversion H; try discriminate.
-  -{ inversion H0.
-     subst. econstructor 1.
-     erewrite app_nil_l. reflexivity.    
-     econstructor.
-   }
-  -{ subst. inv_singleton.
-     eapply struct_equiv_weak_cons_rev.
-     eapply IHG1. eassumption.
-   }
-Qed.
-
-Lemma merge_nil : forall {V : Set} ns,
-    @merge V [] [] ns -> ns = [].
-Proof.
-  induction ns; intros Hm. auto.
-  inversion Hm; try discriminate.
-Qed.
-
-Lemma merge_ex_str : forall {V : Set} G1 G2,
-    struct_equiv_str G1 G2 -> existsT2 G3, @merge V G1 G2 G3.
-Proof.
-  induction G1; intros G2 Hs.
-  inversion Hs. exists []. constructor; reflexivity.
-  discriminate.
-  inversion Hs; try discriminate.
-  inv_singleton. eapply IHG1 in H1.
-  destruct H1 as [G3 H1].
-  eexists ( (Γ1 ++ Γ2, Δ1 ++ Δ2, d) :: G3).
-  econstructor 3; try reflexivity. assumption.
-Qed.
-
-Lemma merge_appLR : forall {V : Set} G1 G2 G3 G,
-    merge G1 G2 G3 ->
-    length G1 = length G2 ->
-    @merge V (G1 ++ G) G2 (G3 ++ G).
-Proof.
-  induction G1; intros until 0; intros Hm Hl.
-  +{ destruct G2. inversion Hm; try discriminate.
-     subst. simpl. econstructor 2; reflexivity.
-     subst. simpl. econstructor 2; reflexivity.
-     discriminate.
-   }
-  +{ destruct G2. discriminate.
-     simpl in Hl. inversion Hl as [Hl'].
-     simpl. destruct G3. inversion Hm; discriminate.
-
-     simpl. inversion Hm; try discriminate.
-     subst. inv_singleton.
-     eapply IHG1 in X.
-     econstructor 3; try reflexivity.
-     eassumption. assumption.
-   }
-Qed.
-
-Lemma merge_appRR : forall {V : Set} G1 G2 G3 G,
-    merge G1 G2 G3 ->
-    length G1 = length G2 ->
-    @merge V (G1) (G2 ++ G) (G3 ++ G).
-Proof.
-  induction G1; intros until 0; intros Hm Hl.
-  +{ destruct G2. inversion Hm; try discriminate.
-     subst. simpl. econstructor 1; reflexivity.
-     subst. simpl. econstructor 1; reflexivity.
-     discriminate.
-   }
-  +{ destruct G2. discriminate.
-     simpl in Hl. inversion Hl as [Hl'].
-     simpl. destruct G3. inversion Hm; discriminate.
-
-     simpl. inversion Hm; try discriminate.
-     subst. inv_singleton.
-     eapply IHG1 in X.
-     econstructor 3; try reflexivity.
-     eassumption. assumption.
-   }
-Qed.
-
-Lemma merge_ex : forall {V : Set} G1 G2,
-    struct_equiv_weak G1 G2 -> existsT2 G3, @merge V G1 G2 G3.
-Proof.
-  intros until 0; intros Hs.
-  inversion Hs; subst;
-  pose proof H0 as H0';
-  eapply struct_equiv_str_length in H0';
-  eapply merge_ex_str in H0;
-  destruct H0 as [G3 H0];
-  exists (G3 ++ ns3).
-
-  eapply merge_appLR; assumption.
-  eapply merge_appRR; assumption.
-Qed.
-
-(* ----------- *)
-(* Equivalence *)
-(* ----------- *)
-
-(* Equality that ignores the last, irrelevant direction. *)
-Inductive LNS_eq {V : Set} : (list (rel (list (PropF V)) * dir)) -> (list (rel (list (PropF V)) * dir)) -> Type :=
-| LNS_eq_nil n1 n2 : n1 = [] -> n2 = [] -> LNS_eq n1 n2
-| LNS_eq_base n1 n2 seq d1 d2 : n1 = [(seq,d1)] -> n2 = [(seq,d2)] -> LNS_eq n1 n2
-| LNS_eq_step ns1 ns2 nseq1 nseq2 : nseq1 = nseq2 -> LNS_eq ns1 ns2 -> LNS_eq (nseq1 :: ns1) (nseq2 :: ns2).
-
-Lemma LNS_eq_eq {V : Set} : forall n1 n2,
-    n1 = n2 -> @LNS_eq V n1 n2.
-Proof.
-  intros n1 n2 H. subst. induction n2.
-  econstructor. reflexivity. reflexivity.
-  destruct n2. destruct a. econstructor 2.  reflexivity. reflexivity.
-  econstructor 3. reflexivity.
-  apply IHn2.
-Qed.
-
-Lemma LNS_eq_cons_same : forall {V : Set} l1 l2 a,
-    LNS_eq (a :: l1) (a :: l2) -> @LNS_eq V l1 l2.
-Proof.
-  intros V l1 l2 a H.
-  inversion H. discriminate.
-  inversion H0. inversion H1. subst.
-  econstructor. reflexivity. reflexivity.
-  subst. assumption.
-Qed.
-
-Lemma LNS_eq_cons : forall {V : Set} l1 l2 a b,
-    LNS_eq (a :: l1) (b :: l2) -> @LNS_eq V l1 l2.
-Proof.
-  intros V l1 l2 a b H.
-  inversion H. discriminate.
-  inversion H0. inversion H1. subst.
-  econstructor. reflexivity. reflexivity.
-  subst. assumption.
-Qed.
-
-Lemma LNS_eq_cons_hd : forall {V : Set} l1 l2 a b,
-    @LNS_eq V (a :: l1) (b :: l2) -> (a = b) + ( (l1 = []) * (l2 = []) ).
-Proof.
-  intros V l1 l2 a b H.
-  inversion H. discriminate.
-  inversion H0. inversion H1. subst.
-  firstorder. subst. firstorder.
-Qed.
-
-Lemma LNS_eq_refl : forall (V : Set) n, @LNS_eq V n n.
-Proof.
-  induction n. constructor; reflexivity.
-  econstructor 3. reflexivity. assumption.
-Qed.
-
-Lemma testing_clear_useless : forall (a b c : nat) (l1 l2 l3 : list nat),
-    a::l1 = b::l2 ->
-    [b] = [c] ->
-    c = a ->
-    l2 = l2 ->
-    [l2] = [l2] ->
-    True.
-Proof.  
-  clear_useless.
-Admitted.
-
-(* ---------------------- *)
-(* Contracted definitions *)
-(* ---------------------- *)
-
-Inductive contracted_multi {T : Type} : list T -> list T -> Type :=
-| cont_multi_refl X : @contracted_multi T X X
-(*| cont_multi_base X Y   : @contracted_gen T X Y -> contracted_multi X Y *)
-| cont_multi_step X Y Z : @contracted_gen T X Y -> contracted_multi Y Z -> contracted_multi X Z.
-
-Inductive contracted_multi_enum {T : Type} : list T -> list T -> nat -> Type :=
-| cont_multi_enum_refl X : @contracted_multi_enum T X X 0
-(*| cont_multi_base X Y   : @contracted_gen T X Y -> contracted_multi X Y *)
-| cont_multi_enum_step X Y Z n : @contracted_gen T X Y -> contracted_multi_enum Y Z n -> contracted_multi_enum X Z (S n).
-
-Lemma cont_multi__enum : forall {T : Type} (X Y : list T),
-    contracted_multi X Y -> existsT2 n, contracted_multi_enum X Y n.
-Proof.
-  intros T X Y Hc.
-  induction Hc. exists 0. eapply cont_multi_enum_refl.
-  destruct IHHc as [n IH].
-  exists (S n). eapply cont_multi_enum_step.
-  eapply c. apply IH.
-Qed.
-
-Lemma cont_multi__enum_rev : forall {T : Type} (X Y : list T) n,
-    contracted_multi_enum X Y n -> contracted_multi X Y.
-Proof.
-  intros T X Y n Hc.
-  induction Hc. eapply cont_multi_refl.
-  eapply cont_multi_step. eapply c.
-  assumption.
-Qed.
-
-Inductive contracted_seqL {T : Type} : ((list T) * (list T) * dir) -> ((list T) * (list T) * dir) -> Type :=
-| cont_seqL X Y Δ d : contracted_multi X Y -> contracted_seqL (X,Δ,d) (Y,Δ,d).
-
-Inductive contracted_seqR {T : Type} : ((list T) * (list T) * dir) -> ((list T) * (list T) * dir) -> Type :=
-| cont_seqR X Y Γ d : contracted_multi X Y -> contracted_seqR (Γ,X,d) (Γ,Y,d).
-
-Inductive contracted_seq {T : Type} : ((list T) * (list T) * dir) -> ((list T) * (list T) * dir) -> Type :=
-| cont_seq_baseL s1 s2 : contracted_seqL s1 s2 -> contracted_seq s1 s2
-| cont_seq_baseR s1 s2  : contracted_seqR s1 s2 -> contracted_seq s1 s2
-| cont_seq_stepL s1 s2 s3 : contracted_seqL s1 s2 -> contracted_seq s2 s3 -> contracted_seq s1 s3
-| cont_seq_stepR s1 s2 s3 : contracted_seqR s1 s2 -> contracted_seq s2 s3 -> contracted_seq s1 s3.
-
-Inductive contracted_nseq {T : Type} : list ((list T) * (list T) * dir) -> list ((list T) * (list T) * dir) -> Type :=
-| cont_nseq_nil  : contracted_nseq [] []
-| cont_nseq_cons s1 s2 ns1 ns2 : contracted_seq s1 s2 -> contracted_nseq ns1 ns2 ->
-                                 contracted_nseq (s1::ns1) (s2::ns2).
-
-Lemma derrec_contracted_multiL : forall {V : Set} Γ1 Γ2 Δ d X Y,
-  contracted_multi Γ1 Γ2 ->
-derrec (LNSKt_rules (V:=V)) (fun _ => False) (X ++ [(Γ1, Δ, d)] ++ Y) ->
-derrec (LNSKt_rules (V:=V)) (fun _ => False) (X ++ [(Γ2, Δ, d)] ++ Y).
-Proof.
-  intros V Γ1 Γ2 Δ d X Y Hc Hd.
-  revert X Y Δ d Hd.
-  induction Hc; intros XX YY Δ d Hd.
-  assumption.
-  eapply IHHc.
-  inversion c; subst;
-  eapply LNSKt_contL_gen.
-  eapply Hd. reflexivity. reflexivity.
-  eapply Hd. reflexivity. reflexivity.
-Qed.
-
-Lemma derrec_contracted_multiR : forall {V : Set} Γ Δ1 Δ2 d X Y,
-  contracted_multi Δ1 Δ2 ->
-derrec (LNSKt_rules (V:=V)) (fun _ => False) (X ++ [(Γ, Δ1, d)] ++ Y) ->
-derrec (LNSKt_rules (V:=V)) (fun _ => False) (X ++ [(Γ, Δ2, d)] ++ Y).
-Proof.
-  intros V Γ Δ1 Δ2 d X Y Hc Hd.
-  revert X Y Γ d Hd.
-  induction Hc; intros XX YY Γ d Hd.
-  assumption.
-  eapply IHHc.
-  inversion c; subst;
-  eapply LNSKt_contR_gen.
-  eapply Hd. reflexivity. reflexivity.
-  eapply Hd. reflexivity. reflexivity.
-Qed.
-
-Lemma derrec_contracted_seqL: forall {V : Set} s1 s2 X Y,
-  contracted_seqL s1 s2 ->
-derrec (LNSKt_rules (V:=V)) (fun _ => False) (X ++ [s1] ++ Y) ->
-derrec (LNSKt_rules (V:=V)) (fun _ => False) (X ++ [s2] ++ Y).
-Proof.
-  intros V s1 s3 X Y Hc Hd.
-  inversion Hc. subst.
-  eapply derrec_contracted_multiL.
-  exact H. assumption.
-Qed.
-
-Lemma derrec_contracted_seqR: forall {V : Set} s1 s2 X Y,
-  contracted_seqR s1 s2 ->
-derrec (LNSKt_rules (V:=V)) (fun _ => False) (X ++ [s1] ++ Y) ->
-derrec (LNSKt_rules (V:=V)) (fun _ => False) (X ++ [s2] ++ Y).
-Proof.
-  intros V s1 s3 X Y Hc Hd.
-  inversion Hc. subst.
-  eapply derrec_contracted_multiR.
-  exact H. assumption.
-Qed.
-  
-Lemma derrec_contracted_seq: forall {V : Set} s1 s2 X Y,
-  contracted_seq s1 s2 ->
-derrec (LNSKt_rules (V:=V)) (fun _ => False) (X ++ [s1] ++ Y) ->
-derrec (LNSKt_rules (V:=V)) (fun _ => False) (X ++ [s2] ++ Y).
-Proof.
-  intros V s1 s2 X Y Hc. revert X Y. 
-  induction Hc as [s1 s2 Hc | s1 s2 Hc | s1 s2 s3 Hc Hc2 | s1 s2 s3 Hc Hc2 ];
-    intros X Y Hd; subst; try eapply IHHc2;
-      (eapply derrec_contracted_seqL; eassumption) ||
-      (eapply derrec_contracted_seqR; eassumption).
-Qed.
-
-Lemma derrec_contracted_nseq: forall {V : Set} ns1 ns2 X Y,
-  contracted_nseq ns1 ns2 ->
-derrec (LNSKt_rules (V:=V)) (fun _ => False) (X ++ ns1 ++ Y) ->
-derrec (LNSKt_rules (V:=V)) (fun _ => False) (X ++ ns2 ++ Y).
-Proof.
-  intros V s1 s2 X Y Hc.
-  revert X Y. 
-  induction Hc as [ | ];
-    intros X Y Hd; subst.
-  +{ eapply Hd. }
-  +{ simpl in Hd. 
-     rewrite cons_singleton in Hd.
-     eapply derrec_contracted_seq in Hd.
-     2 : exact c.
-     simpl. rewrite app_cons_single. eapply IHHc.
-     rewrite <- app_cons_single. exact Hd. }
-Qed.
-
-Lemma contracted_gen_cons : forall {T : Type} Y Z (a : T),
-    contracted_gen Y Z ->
-    contracted_gen (a :: Y) (a :: Z).
-Proof.
-  intros until 0; intros Hc; inversion Hc; subst.
-  rewrite ?app_comm_cons.
-  eapply contracted_genL_I.
-  reflexivity. reflexivity.
-  rewrite ?app_comm_cons.
-  eapply contracted_genR_I.
-  reflexivity. reflexivity.
-Qed.
-
-Lemma contracted_multi_cons : forall {T : Type} Y Z (a : T),
-    contracted_multi Y Z ->
-    contracted_multi (a :: Y) (a :: Z).
-Proof.
-  intros until 0; intros Hc.
-  induction Hc. subst. eapply cont_multi_refl.
-  subst.
-  eapply cont_multi_step. eapply contracted_gen_cons.
-  eapply c.
-  assumption.
-Qed.
-
-Lemma contracted_multi_cons_tl : forall {T : Type} Y Z (a : T),
-    contracted_multi Y Z ->
-    contracted_multi (Y ++ [a]) (Z ++ [a]).
-Proof.
-  intros until 0; intros Hc.
-  induction Hc. eapply cont_multi_refl.
-  inversion c. subst. 
-  eapply cont_multi_step.
-  list_assoc_r'. simpl. eapply contracted_genL_I.
-  reflexivity. reflexivity.
-  do 3 rewrite <- app_assoc in IHHc. assumption.
-
-  subst. eapply cont_multi_step.
-  list_assoc_r'. simpl. eapply contracted_genR_I.
-  reflexivity. reflexivity.
-  do 3 rewrite <- app_assoc in IHHc. assumption.
-Qed.
-
-Lemma contracted_multi_L : forall {T : Type} (X Y Z : list T),
-    contracted_multi Y Z ->
-    contracted_multi (X ++ Y) (X ++ Z).
-Proof.
-  induction X; intros Y Z Hc. assumption.
-  simpl. eapply contracted_multi_cons.
-  apply IHX. apply Hc.
-Qed.
-
-Lemma contracted_multi_R : forall {T : Type} (X Y Z : list T),
-    contracted_multi Y Z ->
-    contracted_multi (Y ++ X) (Z ++ X).
-Proof.
-  induction X; intros Y Z Hc. do 2 rewrite app_nil_r. assumption.
-  rewrite cons_singleton. do 2 rewrite app_assoc.
-  eapply IHX. eapply contracted_multi_cons_tl. assumption.
-Qed.
-
-Lemma contracted_multi_multi : forall {T : Type} Γ X Y Z,
-    @contracted_multi T (X ++ Γ ++ Y ++ Γ ++ Z) (X ++ Γ ++ Y ++ Z).
-Proof.
-  induction X; intros.
-  simpl.
-  list_assoc_l'. eapply contracted_multi_R.
-  list_assoc_r'.
-  revert Y Z.
-  induction Γ; intros Y Z.
-  simpl. rewrite app_nil_r. apply cont_multi_refl.
-  simpl. eapply cont_multi_step.
-  2 :{ eapply contracted_multi_cons. eapply IHΓ. auto. }
-  eapply (contracted_gen__spec a).
-  rewrite (cons_singleton Γ a).
-  do 2 rewrite (cons_singleton (Γ ++ _) a).
-  cont_solve.
-
-  simpl. eapply contracted_multi_cons. apply IHX.
-Qed.
-
-Lemma contracted_multi_double : forall {T : Type} Γ,
-    @contracted_multi T (Γ ++ Γ) Γ.
-Proof.
-  intros T Γ.
-  assert (    @contracted_multi T ([] ++ Γ ++ [] ++ Γ ++ []) ([] ++ Γ ++ [] ++ [])) as Hass.
-  eapply contracted_multi_multi. 
-  repeat rewrite app_nil_r in Hass.  assumption. 
-Qed.
-
-Lemma contracted_seq_double : forall {T : Type} Γ Δ d,
-    @contracted_seq T (Γ ++ Γ, Δ ++ Δ, d) (Γ, Δ, d).
-Proof.
-  intros. econstructor 3.
-  econstructor. eapply contracted_multi_double.
-  econstructor 2. econstructor.
-  eapply contracted_multi_double.
-Qed.
-  
-Lemma contracted_seq_refl : forall {T : Type} s,
-    @contracted_seq T s s.
-Proof.
-  intros T [[Γ Δ] d].
-  econstructor. econstructor.
-  eapply cont_multi_refl.
-Qed.
-
-Lemma contracted_nseq_refl : forall {T : Type} ns,
-    @contracted_nseq T ns ns.
-Proof.
-  induction ns. constructor.
-  constructor. apply contracted_seq_refl.
-  assumption.
-Qed.
-  
-Lemma merge_contracted_nseq : forall {V : Set} G H,
-  @merge V G G H ->
-  contracted_nseq H G.
-Proof.
-  induction G; intros H Hm.
-  eapply merge_nil in Hm. subst. econstructor.
-  inversion Hm; try discriminate.
-  inv_singleton.
-  econstructor. eapply contracted_seq_double.
-  apply IHG. assumption.
-Qed.
-
-Lemma derrec_merge_contracted_multiL : forall {V : Set} X Y Δ d G H,
-    contracted_multi X Y ->
-    derrec (LNSKt_rules (V:=V)) (fun _ : list (rel (list (PropF V)) * dir) => False)
-           (G ++ [(X, Δ, d)] ++ H) ->
-    derrec (LNSKt_rules (V:=V)) (fun _ : list (rel (list (PropF V)) * dir) => False)
-           (G ++ [(Y, Δ, d)] ++ H).
-Proof.
-  intros until 0 ; intros Hc; revert G H; induction Hc; intros G H Hd.
-  assumption.
-  apply IHHc. inversion c; subst.
-  eapply LNSKt_contL_gen; [ eapply Hd | ..];  reflexivity.
-  eapply LNSKt_contL_gen; [ eapply Hd | ..];  reflexivity. 
-Qed.
-
-Lemma derrec_merge_contracted_seqL : forall {V : Set} ss s G H,
-    contracted_seqL ss s ->
-    derrec (LNSKt_rules (V:=V)) (fun _ : list (rel (list (PropF V)) * dir) => False)
-           (G ++ [ss] ++ H) ->
-    derrec (LNSKt_rules (V:=V)) (fun _ : list (rel (list (PropF V)) * dir) => False)
-           (G ++ [s] ++ H).
-Proof.
-  intros until 0; intros Hc.
-  inversion Hc. subst.
-  eapply derrec_merge_contracted_multiL.
-  assumption.
-Qed.
-
-Lemma derrec_merge_contracted_multiR : forall {V : Set} X Y Γ d G H,
-    contracted_multi X Y ->
-    derrec (LNSKt_rules (V:=V)) (fun _ : list (rel (list (PropF V)) * dir) => False)
-           (G ++ [(Γ, X, d)] ++ H) ->
-    derrec (LNSKt_rules (V:=V)) (fun _ : list (rel (list (PropF V)) * dir) => False)
-           (G ++ [(Γ, Y, d)] ++ H).
-Proof.
-  intros until 0 ; intros Hc; revert G H; induction Hc; intros G H Hd.
-  assumption.
-  apply IHHc. inversion c; subst.
-  eapply LNSKt_contR_gen; [ eapply Hd | ..];  reflexivity.
-  eapply LNSKt_contR_gen; [ eapply Hd | ..];  reflexivity. 
-Qed.
-
-Lemma derrec_merge_contracted_seqR : forall {V : Set} ss s G H,
-    contracted_seqR ss s ->
-    derrec (LNSKt_rules (V:=V)) (fun _ : list (rel (list (PropF V)) * dir) => False)
-           (G ++ [ss] ++ H) ->
-    derrec (LNSKt_rules (V:=V)) (fun _ : list (rel (list (PropF V)) * dir) => False)
-           (G ++ [s] ++ H).
-Proof.
-  intros until 0; intros Hc.
-  inversion Hc. subst.
-  eapply derrec_merge_contracted_multiR.
-  assumption.
-Qed.
-
-Lemma derrec_merge_contracted_seq : forall {V : Set} ss s G H,
-    contracted_seq ss s ->
-    derrec (LNSKt_rules (V:=V)) (fun _ => False) (G ++ [ss] ++ H) ->
-    derrec (LNSKt_rules (V:=V)) (fun _ => False) (G ++ [s] ++ H).
-Proof.
-  intros until 0; intros Hc Hd.
-  induction Hc.
-  +{ eapply derrec_merge_contracted_seqL; eassumption. }
-  +{ eapply derrec_merge_contracted_seqR; eassumption. }
-  +{ eapply IHHc.  eapply derrec_merge_contracted_seqL; eassumption. }
-  +{ eapply IHHc.  eapply derrec_merge_contracted_seqR; eassumption. }
-Qed.
-
-Lemma derrec_merge_contracted_nseq_gen : forall {V : Set} H1 H2 G1 G2,
-  contracted_nseq H1 H2 ->
-  derrec (LNSKt_rules (V:=V)) (fun _ => False) (G1 ++ H1 ++ G2) ->
-  derrec (LNSKt_rules (V:=V)) (fun _ => False) (G1 ++ H2 ++ G2).
-Proof.
-  intros until 0; intros Hc; revert G1 G2; induction Hc; intros G1 G2 Hd.
-  inversion Hd. contradiction.
-  subst. assumption.
-
-  simpl in *. rewrite cons_singleton.
-  rewrite cons_singleton in Hd.
-  eapply derrec_merge_contracted_seq.
-  eapply c. rewrite app_assoc.
-  eapply IHHc.
-  rewrite <- app_assoc. assumption.
-Qed.
-  
-Lemma derrec_merge_contracted_nseq : forall {V : Set} G H,
-  contracted_nseq H G ->
-  derrec (LNSKt_rules (V:=V)) (fun _ => False) H ->
-  derrec (LNSKt_rules (V:=V)) (fun _ => False) G.
-Proof.
-  intros until 0; intros Hc Hd.
-  assert (G =  ([] ++ G ++ [])) as Hass1.
-  rewrite app_nil_r. reflexivity.
-  rewrite Hass1. eapply derrec_merge_contracted_nseq_gen.
-  eapply Hc.
-  rewrite app_nil_r. assumption.
-Qed.
-  
-Lemma derrec_merge_nseq_double : forall {V : Set} G H,
-  merge G G H ->
-  derrec (LNSKt_rules (V:=V)) (fun _ => False) H ->
-  derrec (LNSKt_rules (V:=V)) (fun _ => False) G.
-Proof.
-  intros until 0; intros Hm Hd.
-  eapply derrec_merge_contracted_nseq.
-  eapply merge_contracted_nseq. eassumption.
-  assumption.
-Qed.
-
-Lemma LNSKt_contraction_cor : forall (V : Set) G1 G2 G3,
-    merge G1 G1 G3 ->
-    derrec (LNSKt_rules (V:=V)) (fun _ => False) (G3 ++ G2) ->
-    derrec (LNSKt_rules (V:=V)) (fun _ => False) (G1 ++ G2).
-Proof.
-  intros until 0; intros Hm Hd.
-  rewrite <- app_nil_l.
-  rewrite <- app_nil_l in Hd.
-  eapply derrec_merge_contracted_nseq_gen.
-  eapply merge_contracted_nseq. eassumption.
-  assumption.
-Qed.
-
-(* --------------------------------- *)
-(* CUT ADMISSIBILITY AND ELIMINATION *)
-(* --------------------------------- *)
 
 Definition can_gen_cut {V : Set}
   (rules : rlsT (list (rel (list (PropF V)) * dir))) ns1 ns2 :=
@@ -856,13 +27,6 @@ Definition can_gen_cut {V : Set}
     struct_equiv_str G1 G2 ->
     derrec rules (fun _ => False) (G3 ++ [(Γ1++Γ2, Δ1++Δ2, d)]).
 
-(* TODO: To fill in proof, based off Lemma 16 of paper. *)
-Theorem LNSKt_cut_admissibility : forall (V : Set) ns1 ns2
-  (D1 : derrec (@LNSKt_rules V) (fun _ => False) ns1)
-  (D2 : derrec (@LNSKt_rules V) (fun _ => False) ns2),
-      can_gen_cut (@LNSKt_rules V) ns1 ns2.
-Admitted.
-
 Definition can_gen_cut_simpl {V : Set}
   (rules : rlsT (list (rel (list (PropF V)) * dir))) ns1 ns2 :=
   forall G seq1 seq2 (d : dir) Γ1 Γ2 Δ1 Δ2 A,
@@ -870,7 +34,149 @@ Definition can_gen_cut_simpl {V : Set}
     ns2 = G ++ [(seq2, d)] -> seq2 = pair (Γ2++[A]) Δ2 ->
     derrec rules (fun _ => False) (G ++ [(Γ1++Γ2, Δ1++Δ2, d)]).
 
-Theorem LNSKt_cut_elimination_simpl : forall (V : Set) ns1 ns2
+
+(* ----------------- *)
+(* CUT ADMISSIBILITY *)
+(* ----------------- *)
+
+Definition ht := derrec_height.
+
+
+Definition size {V : Set} (A : PropF V) := 0.
+Print LNSKt_rules.
+Print prop.
+Print princrule_pfc.
+Print derrec.
+
+
+Parameter V : Set.
+Parameter p q : V.
+Definition P := Var p.
+Definition Q := Var q.
+Print PropF.
+Check (dlNil (@LNSKt_rules V) (fun _ => False)).
+Definition d0 := (dlNil (@LNSKt_rules V) (fun _ => False)).
+Print derI.
+Print LNSKt_rules.
+
+Definition d1 : derrec (LNSKt_rules (V:=V)) (fun _ : list (rel (list (PropF V)) * dir) => False) [([Imp P Q ; Q ; P], [Q], fwd)].
+  eapply derI.
+  eapply prop.
+  rewrite <- app_nil_l.
+  rewrite <- nslcext_def.
+  eapply NSlcctxt.
+  eapply Sctxt_eq;
+  [ | rewrite cons_singleton;  rewrite (cons_singleton _ Q);  reflexivity |
+    rewrite <- (app_nil_l [Q]); rewrite <- (app_nil_r [Q]); reflexivity | ..].
+  eapply Id_pfc.
+  reflexivity.
+  apply dlNil.
+Qed.
+
+Definition d1' : derrec (LNSKt_rules (V:=V)) (fun _ : list (rel (list (PropF V)) * dir) => False) (nslcext [] fwd (seqext [Imp P Q] [P] [] [] ([Q],[Q]))). 
+  eapply derI.
+  eapply prop.
+  eapply NSlcctxt.
+  eapply Sctxt.
+  eapply Id_pfc.
+  apply dlNil.
+Qed.
+
+Definition d1'' : derrec (LNSKt_rules (V:=V)) (fun _ : list (rel (list (PropF V)) * dir) => False) [([Imp P Q ; Q ; P], [Q], fwd)].
+  rewrite <- app_nil_l.
+  rewrite <- nslcext_def.
+  rewrite cons_singleton.
+  rewrite <- (app_nil_l [Q]).
+  rewrite <- (app_nil_r [Q]).
+  rewrite (cons_singleton _ Q).
+  rewrite <- seqext_def.
+  apply d1'.
+Qed.
+
+Definition d2 : derrec (LNSKt_rules (V:=V)) (fun _ : list (rel (list (PropF V)) * dir) => False) [([Imp P Q ; P], [Q ; P], fwd)].
+  eapply derI.
+  eapply prop.
+  rewrite <- app_nil_l.
+  rewrite <- nslcext_def.
+  eapply NSlcctxt.
+  eapply Sctxt_eq;
+  [ | erewrite app_nil_r; rewrite cons_singleton; reflexivity |
+    erewrite app_nil_r; rewrite cons_singleton; reflexivity |..].
+  eapply Id_pfc.
+  reflexivity.
+  apply dlNil.
+Qed.
+
+Definition d3 : derrec (LNSKt_rules (V:=V)) (fun _ => False) [([Imp P Q; P], [Q], fwd)].
+  eapply derI.
+  eapply prop.
+  rewrite <- app_nil_l.
+  rewrite <- nslcext_def.
+  eapply NSlcctxt.
+  eapply Sctxt_eq.
+  eapply ImpL_pfc.
+  rewrite cons_singleton.
+  rewrite <- (app_nil_l (_ ++ [P])).
+  reflexivity.
+  simpl. erewrite app_nil_r. reflexivity.
+  reflexivity.
+  eapply dlCons. eapply d1.
+  eapply dlCons. eapply d2.
+  eapply dlNil.
+Qed.
+
+Inductive principal1 {V : Set} {rules : rlsT (list (rel (list (PropF V)) * dir))}
+          {prems} {G} (D : derrec rules prems G) (A : PropF V) :=
+| princ_prop  
+
+
+Definition principal' {V : Set} {rules : rlsT (list (rel (list (PropF V)) * dir))}
+           {prems : X -> Type} {G} (D : @derrec X rules prems G) (A : PropF V) := True.
+
+Definition SR_wb_fwd (n m : nat) := forall {V : Set} rules
+    G Γ Δ H Σ Π I (A : PropF V)
+  (D1 : derrec rules (fun _ => False) (G ++ [(Γ, Δ ++ [WBox A],fwd)]))
+  (D2 : derrec rules (fun _ => False) (H ++ [(Σ ++ [WBox A], Π, fwd)] ++ I)),
+        principal D1 (WBox A) ->
+        ((ht _ _ _ _ D1) + (ht _ _ _ _ D2))%nat <= m ->
+        merge G H I ->
+        (exists (D3 : derrec rules (fun _ => False)
+                       (I ++ [(Γ ++ Σ, Δ ++ Π, fwd)] ++
+                           [([],[A],fwd)] )), True) ->
+        size (WBox A) <= n ->
+        exists (D4 : derrec rules (fun _ => False)
+                       (I ++ [(Γ ++ Σ, Δ ++ Π, fwd)] ++ I )), True .
+
+Definition SR_wb_bac (n m : nat) := forall {V : Set} rules
+    G Γ Δ H Σ Π I (A : PropF V)
+  (D1 : derrec rules (fun _ => False) (G ++ [(Γ, Δ ++ [WBox A],bac)]))
+  (D2 : derrec rules (fun _ => False) (H ++ [(Σ ++ [WBox A], Π, bac)] ++ I)),
+        principal D1 (WBox A) ->
+        ((ht _ _ _ _ D1) + (ht _ _ _ _ D2))%nat <= m ->
+        merge G H I ->
+        (exists (D3 : derrec rules (fun _ => False)
+                       (I ++ [(Γ ++ Σ, Δ ++ Π, bac)] ++
+                           [([],[A],fwd)] )), True) ->
+        size (WBox A) <= n ->
+        exists (D4 : derrec rules (fun _ => False)
+                       (I ++ [(Γ ++ Σ, Δ ++ Π, bac)] ++ I )), True .
+
+
+Theorem Lemma_Sixteen :
+
+
+
+
+
+(* TODO: To fill in proof, based off Lemma 16 of paper. *)
+Theorem LNSKt_cut_admissibility : forall (V : Set) ns1 ns2
+  (D1 : derrec (@LNSKt_rules V) (fun _ => False) ns1)
+  (D2 : derrec (@LNSKt_rules V) (fun _ => False) ns2),
+      can_gen_cut (@LNSKt_rules V) ns1 ns2.
+Admitted.
+
+(* Follows from LNSKt_cut_admissibility. *)
+Theorem LNSKt_cut_admissibility_simpl : forall (V : Set) ns1 ns2
   (D1 : derrec (@LNSKt_rules V) (fun _ => False) ns1)
   (D2 : derrec (@LNSKt_rules V) (fun _ => False) ns2),
     can_gen_cut_simpl (@LNSKt_rules V) ns1 ns2.
@@ -878,7 +184,7 @@ Proof.
   intros. unfold can_gen_cut_simpl.
   intros. subst.
   destruct (@merge_ex V _ _ (struct_equiv_weak_refl G)) as [G3 HG3].  
-  eapply LNSKt_contraction_cor.
+  eapply derrec_mergeL.
   eassumption.
   eapply LNSKt_cut_admissibility in D2. 2 : exact D1.
   unfold can_gen_cut in D2.
@@ -887,68 +193,18 @@ Proof.
   apply struct_equiv_str_refl.
 Qed.
 
-Lemma external_weakeningR : forall {V : Set} ns1 ns2,
-    derrec (@LNSKt_rules V) (fun _ => False) ns1 ->
-    derrec (@LNSKt_rules V) (fun _ => False) (ns1 ++ ns2).
-Proof.
-  intros V ns1 ns2. revert ns1.
-  induction ns2; intros ns1 Hder.
-  rewrite app_nil_r. assumption.
-  rewrite app_cons_single. eapply IHns2.
-  eapply derI. eapply nEW. constructor.
-  destruct a. destruct r. constructor.
-  unfold nslclext. simpl. rewrite app_nil_r.
-  constructor. eapply Hder.
-  eapply dlNil.
-Qed.
 
+(* --------------- *)
 (* CUT ELIMINATION *)
+(* --------------- *)
 
 Inductive Cut_rule {V : Set} : rlsT (list (rel (list (PropF V)) * dir)) :=
 | Cut : forall Γ1 Γ2 Δ1 Δ2 d A, Cut_rule ([[(Γ1,Δ1++[A],d)]] ++ [[(Γ2++[A],Δ2,d)]]) [(Γ1++Γ2,Δ1++Δ2, d)].
 
+(* LNSKt with cut: rules "WithOut Cut" (_woc) and "With Cut" (_wc). *)
 Inductive LNSKt_cut_rules {V : Set} : rlsT (list (rel (list (PropF V)) * dir)) :=
 | LNSKt_rules_woc : forall ps c, LNSKt_rules ps c -> LNSKt_cut_rules ps c
 | LNSKt_rules_wc  : forall ps c, nslclrule (@Cut_rule V) ps c -> LNSKt_cut_rules ps c.
-
-Theorem strong_induction_Prop:
-forall P : nat -> Prop,
-(forall n : nat, (forall k : nat, (k < n -> P k)) -> P n) ->
-forall n : nat, P n.
-Proof.
-  intros P Hind.
-  assert ((forall n k, k <= n -> P k) -> forall n, P n) as Hass.
-    intros HH n. eapply HH. eapply le_n.
-  eapply Hass. clear Hass.
-    induction n; intros k Hk. eapply PeanoNat.Nat.le_0_r in Hk.
-    subst. eapply Hind. firstorder.
-
-    eapply Lt.le_lt_or_eq in Hk. destruct Hk.
-    eapply IHn. inversion H. apply le_n. subst. 
-    apply Le.le_Sn_le in H1.
-    assumption.
-    subst. apply Hind. firstorder.
-Qed.
-
-Theorem strong_induction:
-forall P : nat -> Type,
-(forall n : nat, (forall k : nat, (k < n -> P k)) -> P n) ->
-forall n : nat, P n.
-Proof.
-  intros P Hind.
-  assert ((forall n k, k <= n -> P k) -> forall n, P n) as Hass.
-    intros HH n. eapply HH. eapply le_n.
-  eapply Hass. clear Hass.
-  induction n; intros k Hk.
-    eapply PeanoNat.Nat.le_0_r in Hk.
-    subst. eapply Hind. firstorder.
-    eapply Compare_dec.le_lt_eq_dec in Hk. 
-    destruct Hk.
-    eapply IHn. inversion l. apply le_n. subst. 
-    apply Le.le_Sn_le in H0.
-    assumption.
-    subst. apply Hind. firstorder.
-Qed.
 
 Lemma dersrec_derrec_height : forall {V : Set} rules ps p 
     (ds : dersrec rules (fun _ : list (rel (list (PropF V)) * dir) => False) ps)
@@ -1012,7 +268,7 @@ Proof.
   intros V ns H.
   remember (derrec_height H) as n.
   revert Heqn. revert H. revert ns.
-  induction n using strong_induction.
+  induction n using lt_wf_indT. 
   destruct n.
   +{ intros ns H Heqn. destruct H. contradiction.
      simpl in Heqn. discriminate.
@@ -1041,7 +297,7 @@ Proof.
          pose proof (@merge_ex V) as XX.
          edestruct XX as [G3 HG3].
          eapply struct_equiv_weak_refl.
-         eapply LNSKt_contraction_cor.
+         eapply derrec_mergeL.
          exact HG3.
          eapply LNSKt_cut_admissibility; [ | | reflexivity | reflexivity | reflexivity | reflexivity | exact HG3 | ..].
          +++{ eapply X. 2 : reflexivity. Unshelve.
@@ -1061,4 +317,4 @@ Proof.
    }
 Defined.
 
-Print Assumptions LNSKt_cut_elimination.
+Print Assumptions LNSKt_cut_elimination. 
