contractedT.v
@@ -1,0 +1,407 @@
+Require Import List.
+Require Import existsT.
+Require Import List_lemmasT.
+Require Import gen genT lntacsT.
+Require Import lntT.
+
+Set Implicit Arguments.
+Import ListNotations.
+
+(* Contains definitions and lemmas for ... *)
+
+Inductive contracted {T} : list T -> list T -> Type :=
+  | contracted_I : forall a (X Y A B : list T), X = (A ++ [a;a] ++ B) -> 
+    Y = (A ++ [a] ++ B) -> contracted X Y.
+
+Lemma contracted_I': forall T a (A B : list T),
+   contracted (A ++ [a;a] ++ B) (A ++ [a] ++ B).
+Proof.  intros.  eapply contracted_I ; reflexivity. Qed.
+
+Inductive contracted_gen {T} : list T -> list T -> Type :=
+| contracted_genL_I : forall a (X Y A B C : list T),
+    X = (A ++ [a] ++ B ++ [a] ++ C) -> 
+    Y = (A ++ [a] ++ B ++ C) -> contracted_gen X Y
+| contracted_genR_I : forall a (X Y A B C : list T),
+    X = (A ++ [a] ++ B ++ [a] ++ C) -> 
+    Y = (A ++ B ++ [a] ++ C) -> contracted_gen X Y.
+
+Inductive contracted_gen_spec {T} (a : T) : list T -> list T -> Type :=
+| contracted_genL_spec_I : forall (X Y A B C : list T),
+    X = (A ++ [a] ++ B ++ [a] ++ C) -> 
+    Y = (A ++ [a] ++ B ++ C) -> contracted_gen_spec a X Y
+| contracted_genR_spec_I : forall (X Y A B C : list T),
+    X = (A ++ [a] ++ B ++ [a] ++ C) -> 
+    Y = (A ++ B ++ [a] ++ C) -> contracted_gen_spec a X Y.
+
+Lemma contracted_genL_I': forall T a (A B C : list T),
+   contracted_gen (A ++ [a] ++ B ++ [a] ++ C) (A ++ [a] ++ B ++ C).
+Proof.  intros.  eapply contracted_genL_I ; reflexivity. Qed.
+
+Lemma contracted_genR_I': forall T a (A B C : list T),
+   contracted_gen (A ++ [a] ++ B ++ [a] ++ C) (A ++ B ++ [a] ++ C).
+Proof.  intros.  eapply contracted_genR_I ; reflexivity. Qed.
+
+Lemma contracted_genR_spec_I': forall T a (A B C : list T),
+   contracted_gen_spec a (A ++ [a] ++ B ++ [a] ++ C) (A ++ B ++ [a] ++ C).
+Proof.  intros.  eapply contracted_genR_spec_I ; reflexivity. Qed.
+
+Lemma contracted_genL_spec_I': forall T a (A B C : list T),
+   contracted_gen_spec a (A ++ [a] ++ B ++ [a] ++ C) (A ++ [a] ++ B ++ C).
+Proof.  intros.  eapply contracted_genL_spec_I ; reflexivity. Qed.
+
+Lemma contracted_gen__spec : forall {T} (a : T) l1 l2,
+    contracted_gen_spec a l1 l2 -> contracted_gen l1 l2.
+Proof.
+  intros until 0; intros H. inversion H;
+  [eapply contracted_genL_I |
+   eapply contracted_genR_I].
+  1,3 : apply H0.
+  all : apply H1.
+Qed.
+
+(* ------------------- *)
+(* CONTRACTION TACTICS *)
+(* ------------------- *)
+
+Lemma cont_L: forall T X Y Z,
+  contracted X (Y : list T) -> contracted (Z ++ X) (Z ++ Y).
+Proof.
+  intros until 0; intros H. destruct H. subst. 
+  rewrite !(app_assoc Z). apply contracted_I'.
+Qed.
+
+Lemma cont_R: forall T X Y Z,
+  contracted X (Y : list T) -> contracted (X ++ Z) (Y ++ Z).
+Proof.
+  intros until 0; intros H. destruct H. subst.
+  rewrite <- !app_assoc. apply contracted_I'. 
+Qed.
+
+Lemma cont_gen_L: forall T X Y Z,
+  contracted_gen X (Y : list T) -> contracted_gen (Z ++ X) (Z ++ Y).
+Proof.
+  intros until 0; intros H. destruct H; subst; rewrite !(app_assoc Z).
+  apply contracted_genL_I'.
+  apply contracted_genR_I'.
+Qed.
+
+Lemma cont_gen_R: forall T X Y Z,
+  contracted_gen X (Y : list T) -> contracted_gen (X ++ Z) (Y ++ Z).
+Proof.
+  intros until 0; intros H. destruct H; subst; rewrite <- !app_assoc.
+  apply contracted_genL_I'. 
+  apply contracted_genR_I'. 
+Qed.
+
+Lemma cont_gen_spec_basic : forall T (a : T),
+    contracted_gen_spec a ([a]++[a]) [a].
+Proof.
+  intros. change ([a] ++ [a]) with ([] ++ [a] ++ [] ++ [a] ++ []).
+  change ([a]) with ([] ++ [a] ++ [] ++ []) at 3.
+  apply contracted_genL_spec_I'.
+Qed.
+  
+Lemma cont_gen_spec_L: forall T a X Y Z,
+  contracted_gen_spec a X (Y : list T) -> contracted_gen_spec a (Z ++ X) (Z ++ Y).
+Proof.
+  intros until 0; intros H. destruct H; subst; rewrite !(app_assoc Z).
+  apply contracted_genL_spec_I'.
+  apply contracted_genR_spec_I'.
+Qed.
+
+Lemma cont_gen_spec_R: forall T a X Y Z,
+  contracted_gen_spec a X (Y : list T) -> contracted_gen_spec a (X ++ Z) (Y ++ Z).
+Proof.
+  intros until 0; intros H. destruct H; subst; rewrite <- !app_assoc.
+  apply contracted_genL_spec_I'. 
+  apply contracted_genR_spec_I'. 
+Qed.
+
+Lemma cont_gen_spec_rem_sml_L : forall T (a : T) Z,
+    contracted_gen_spec a ([a] ++ Z ++ [a]) ([a] ++ Z).
+Proof.
+  intros.
+  change ([a] ++ Z ++ [a]) with ([] ++ [a] ++ Z ++ [a] ++ []).
+  replace ([a] ++ Z) with ([] ++ [a] ++ Z ++ []).
+  apply contracted_genL_spec_I'. rewrite app_nil_r. reflexivity.
+Qed.
+
+Lemma cont_gen_spec_rem_sml_R : forall T (a : T) Z,
+    contracted_gen_spec a ([a] ++ Z ++ [a]) (Z ++ [a]).
+Proof.
+  intros.
+  change ([a] ++ Z ++ [a]) with ([] ++ [a] ++ Z ++ [a] ++ []).
+  change (Z ++ [a]) with ([] ++ Z ++ [a] ++ []).
+  apply contracted_genR_spec_I'.
+Qed.
+
+Lemma cont_cons: forall T (x : T) Y Z,
+  contracted Y Z -> contracted (x :: Y) (x :: Z).
+Proof.
+  intros until 0; intros H. inversion H.
+  subst. list_assoc_l.
+  rewrite <- !app_assoc. apply contracted_I'.
+Qed.
+
+Lemma contracted_gen_in1: forall {T} (a : T) A Γ1 C H5,
+    InT a C ->
+ contracted_gen (A ++ [a] ++ Γ1 ++ C ++ H5) (A ++ Γ1 ++ C ++ H5).
+Proof.
+  intros until 0; intros H. apply InT_split in H.
+  destruct H as [l1 [l2 H]].
+  subst.  list_assoc_r'.
+  simpl.
+  do 2 change (a :: (?x ++ ?y)) with ([a] ++ (x ++ y)).
+  eapply contracted_genR_I.
+  do 2 apply applI.
+  rewrite app_assoc.  reflexivity.
+  list_assoc_r'. reflexivity.
+Qed.
+
+Lemma contracted_gen_in2: forall {T} (a : T) A Γ1 C,
+    InT a Γ1 ->
+ contracted_gen (A ++ [a] ++ Γ1 ++ C) (A ++ Γ1 ++ C).
+Proof.
+  intros until 0; intros H. apply InT_split in H.
+  destruct H as [l1 [l2 H]].
+  subst.   list_assoc_r'.
+  simpl.
+  change (a :: ?x) with ([a] ++ x).
+  eapply contracted_genR_I.
+  do 3 apply applI.
+  2 : do 3 apply applI.
+  all : reflexivity.
+Qed.
+
+Lemma contracted_gen_in3: forall {T} (a : T) A Γ1 C,
+    InT a Γ1 ->
+contracted_gen (A ++ Γ1 ++ [a] ++ C) (A ++ Γ1 ++ C).
+Proof.
+  intros until 0; intros H. apply InT_split in H.
+  destruct H as [l1 [l2 H]].
+  subst.   list_assoc_r'.
+  simpl.
+  change (a :: ?x) with ([a] ++ x).
+  eapply contracted_genL_I.
+  rewrite app_assoc.
+  do 3 apply applI. reflexivity.
+  apps_eq_tac.
+Qed.
+
+Lemma contracted_gen_in4: forall {T} (a : T) A Γ1 H5 C,
+    InT a Γ1 ->
+    contracted_gen (A ++ Γ1 ++ H5 ++ [a] ++ C) (A ++ Γ1 ++ H5 ++ C).
+Proof.
+  intros until 0; intros H. apply InT_split in H.
+  destruct H as [l1 [l2 H]].
+  subst.
+  change (a :: ?x) with ([a] ++ x).
+  assoc_mid [a].
+  eapply contracted_genL_I.
+  do 2 apply applI.
+  assoc_mid [a]. reflexivity.
+  apps_eq_tac.
+Qed.
+
+Ltac cont_rem_head :=
+  list_assoc_r'; rewrite ?app_comm_cons;
+  repeat match goal with
+  | [ |- contracted_gen_spec ?a ?l1 ?l2 ] =>
+    (tryif check_app_head l1 [a] then idtac else apply cont_gen_spec_L)
+  end.
+
+Ltac cont_rem_tail :=
+  list_assoc_l'; rewrite ?app_comm_cons;
+  repeat match goal with
+  | [ |- contracted_gen_spec ?a ?l1 ?l2 ] =>
+    (tryif check_app_tail l1 [a] then idtac else apply cont_gen_spec_R)
+         end.
+
+Ltac cont_rem_mid_simp :=
+  apply cont_gen_spec_basic || apply cont_gen_spec_rem_sml_L
+|| apply cont_gen_spec_rem_sml_R.
+
+Ltac cont_gen_spec_app_brac_mid_L :=
+  match goal with
+  | [ |- contracted_gen_spec _ ?l1 ?l2 ] => app_bracket_middle_arg l1
+  end.
+
+Ltac cont_gen_spec_app_brac_mid_R :=
+  match goal with
+  | [ |- contracted_gen_spec _ ?l1 ?l2 ] => app_bracket_middle_arg l2
+  end.
+
+Ltac cont_gen_spec_app_brac_mid :=
+  cont_gen_spec_app_brac_mid_L; cont_gen_spec_app_brac_mid_R.
+
+(* Use this one *)
+Ltac cont_solve :=
+  cont_rem_head; cont_rem_tail;
+  list_assoc_r_single; repeat cont_gen_spec_app_brac_mid;
+  cont_rem_mid_simp.
+
+Ltac cont_solve' :=
+  cont_rem_head; cont_rem_tail;
+  list_assoc_r_single; cont_gen_spec_app_brac_mid;
+  cont_rem_mid_simp.
+
+Inductive contracted_multi {T : Type} : list T -> list T -> Type :=
+| cont_multi_refl X : @contracted_multi T X X
+(*| cont_multi_base X Y   : @contracted_gen T X Y -> contracted_multi X Y *)
+| cont_multi_step X Y Z : @contracted_gen T X Y -> contracted_multi Y Z -> contracted_multi X Z.
+
+Inductive contracted_multi_enum {T : Type} : list T -> list T -> nat -> Type :=
+| cont_multi_enum_refl X : @contracted_multi_enum T X X 0
+(*| cont_multi_base X Y   : @contracted_gen T X Y -> contracted_multi X Y *)
+| cont_multi_enum_step X Y Z n : @contracted_gen T X Y -> contracted_multi_enum Y Z n -> contracted_multi_enum X Z (S n).
+
+Lemma cont_multi__enum : forall {T : Type} (X Y : list T),
+    contracted_multi X Y -> existsT2 n, contracted_multi_enum X Y n.
+Proof.
+  intros T X Y Hc.
+  induction Hc. exists 0. eapply cont_multi_enum_refl.
+  destruct IHHc as [n IH].
+  exists (S n). eapply cont_multi_enum_step.
+  eapply c. apply IH.
+Qed.
+
+Lemma cont_multi__enum_rev : forall {T : Type} (X Y : list T) n,
+    contracted_multi_enum X Y n -> contracted_multi X Y.
+Proof.
+  intros T X Y n Hc.
+  induction Hc. eapply cont_multi_refl.
+  eapply cont_multi_step. eapply c.
+  assumption.
+Qed.
+
+Inductive contracted_seqL {T : Type} : ((list T) * (list T) * dir) -> ((list T) * (list T) * dir) -> Type :=
+| cont_seqL X Y Δ d : contracted_multi X Y -> contracted_seqL (X,Δ,d) (Y,Δ,d).
+
+Inductive contracted_seqR {T : Type} : ((list T) * (list T) * dir) -> ((list T) * (list T) * dir) -> Type :=
+| cont_seqR X Y Γ d : contracted_multi X Y -> contracted_seqR (Γ,X,d) (Γ,Y,d).
+
+Inductive contracted_seq {T : Type} : ((list T) * (list T) * dir) -> ((list T) * (list T) * dir) -> Type :=
+| cont_seq_baseL s1 s2 : contracted_seqL s1 s2 -> contracted_seq s1 s2
+| cont_seq_baseR s1 s2  : contracted_seqR s1 s2 -> contracted_seq s1 s2
+| cont_seq_stepL s1 s2 s3 : contracted_seqL s1 s2 -> contracted_seq s2 s3 -> contracted_seq s1 s3
+| cont_seq_stepR s1 s2 s3 : contracted_seqR s1 s2 -> contracted_seq s2 s3 -> contracted_seq s1 s3.
+
+Inductive contracted_nseq {T : Type} : list ((list T) * (list T) * dir) -> list ((list T) * (list T) * dir) -> Type :=
+| cont_nseq_nil  : contracted_nseq [] []
+| cont_nseq_cons s1 s2 ns1 ns2 : contracted_seq s1 s2 -> contracted_nseq ns1 ns2 ->
+                                 contracted_nseq (s1::ns1) (s2::ns2).
+
+Lemma contracted_gen_cons : forall {T : Type} Y Z (a : T),
+    contracted_gen Y Z ->
+    contracted_gen (a :: Y) (a :: Z).
+Proof.
+  intros until 0; intros Hc; inversion Hc; subst.
+  rewrite ?app_comm_cons.
+  eapply contracted_genL_I.
+  reflexivity. reflexivity.
+  rewrite ?app_comm_cons.
+  eapply contracted_genR_I.
+  reflexivity. reflexivity.
+Qed.
+
+Lemma contracted_multi_cons : forall {T : Type} Y Z (a : T),
+    contracted_multi Y Z ->
+    contracted_multi (a :: Y) (a :: Z).
+Proof.
+  intros until 0; intros Hc.
+  induction Hc. subst. eapply cont_multi_refl.
+  subst.
+  eapply cont_multi_step. eapply contracted_gen_cons.
+  eapply c.
+  assumption.
+Qed.
+
+Lemma contracted_multi_cons_tl : forall {T : Type} Y Z (a : T),
+    contracted_multi Y Z ->
+    contracted_multi (Y ++ [a]) (Z ++ [a]).
+Proof.
+  intros until 0; intros Hc.
+  induction Hc. eapply cont_multi_refl.
+  inversion c. subst. 
+  eapply cont_multi_step.
+  list_assoc_r'. simpl. eapply contracted_genL_I.
+  reflexivity. reflexivity.
+  do 3 rewrite <- app_assoc in IHHc. assumption.
+
+  subst. eapply cont_multi_step.
+  list_assoc_r'. simpl. eapply contracted_genR_I.
+  reflexivity. reflexivity.
+  do 3 rewrite <- app_assoc in IHHc. assumption.
+Qed.
+
+Lemma contracted_multi_L : forall {T : Type} (X Y Z : list T),
+    contracted_multi Y Z ->
+    contracted_multi (X ++ Y) (X ++ Z).
+Proof.
+  induction X; intros Y Z Hc. assumption.
+  simpl. eapply contracted_multi_cons.
+  apply IHX. apply Hc.
+Qed.
+
+Lemma contracted_multi_R : forall {T : Type} (X Y Z : list T),
+    contracted_multi Y Z ->
+    contracted_multi (Y ++ X) (Z ++ X).
+Proof.
+  induction X; intros Y Z Hc. do 2 rewrite app_nil_r. assumption.
+  rewrite cons_singleton. do 2 rewrite app_assoc.
+  eapply IHX. eapply contracted_multi_cons_tl. assumption.
+Qed.
+
+Lemma contracted_multi_multi : forall {T : Type} Γ X Y Z,
+    @contracted_multi T (X ++ Γ ++ Y ++ Γ ++ Z) (X ++ Γ ++ Y ++ Z).
+Proof.
+  induction X; intros.
+  simpl.
+  list_assoc_l'. eapply contracted_multi_R.
+  list_assoc_r'.
+  revert Y Z.
+  induction Γ; intros Y Z.
+  simpl. rewrite app_nil_r. apply cont_multi_refl.
+  simpl. eapply cont_multi_step.
+  2 :{ eapply contracted_multi_cons. eapply IHΓ. auto. }
+  eapply (@contracted_gen__spec _ a).
+  rewrite (cons_singleton Γ a).
+  do 2 rewrite (cons_singleton (Γ ++ _) a).
+  cont_solve.
+
+  simpl. eapply contracted_multi_cons. apply IHX.
+Qed.
+
+Lemma contracted_multi_double : forall {T : Type} Γ,
+    @contracted_multi T (Γ ++ Γ) Γ.
+Proof.
+  intros T Γ.
+  assert (    @contracted_multi T ([] ++ Γ ++ [] ++ Γ ++ []) ([] ++ Γ ++ [] ++ [])) as Hass.
+  eapply contracted_multi_multi. 
+  repeat rewrite app_nil_r in Hass.  assumption. 
+Qed.
+
+Lemma contracted_seq_double : forall {T : Type} Γ Δ d,
+    @contracted_seq T (Γ ++ Γ, Δ ++ Δ, d) (Γ, Δ, d).
+Proof.
+  intros. econstructor 3.
+  econstructor. eapply contracted_multi_double.
+  econstructor 2. econstructor.
+  eapply contracted_multi_double.
+Qed.
+  
+Lemma contracted_seq_refl : forall {T : Type} s,
+    @contracted_seq T s s.
+Proof.
+  intros T [[Γ Δ] d].
+  econstructor. econstructor.
+  eapply cont_multi_refl.
+Qed.
+
+Lemma contracted_nseq_refl : forall {T : Type} ns,
+    @contracted_nseq T ns ns.
+Proof.
+  induction ns. constructor.
+  constructor. apply contracted_seq_refl.
+  assumption.
+Qed.
