ind_lex.v
@@ -1,0 +1,70 @@
+Require Import Lexicographic_Product.
+Require Import Relation_Operators.
+Require Import Wf_nat.
+Require Import Inverse_Image.
+
+(* Type version (for P : nat -> Type) of lt_wf_ind, still based off Prop lt. *)
+Lemma lt_wf_indT :
+  forall n (P:nat -> Type), (forall n, (forall m, m < n -> P m) -> P n) -> P n.
+Proof.
+  induction n; intros P IH.
+  apply IH. intros m Hm.
+  apply PeanoNat.Nat.nlt_0_r in Hm.
+  contradiction.
+
+  apply IHn.
+  intros u Hu.
+  apply IH.
+  intros v Hv.
+  destruct v.
+  apply IH. intros m Hm.
+  apply PeanoNat.Nat.nlt_0_r in Hm. contradiction.
+  apply Lt.lt_S_n in Hv.
+  apply Hu in Hv. assumption.
+Qed.
+
+(* The following was adapted from Pierre Casteran's answer to this coq-club question:
+https://coq-club.inria.narkive.com/7Mts7wuN/how-to-show-lexicographic-product-of-three-well-founded-sets-is-well-founded
+ *)
+
+Definition dep2 := sigT (A:=nat) (fun a => nat).
+
+Definition mk2 :=
+(fun H : nat * nat => let (p, q) := H in existT (fun _ : nat => nat) p q).
+(*  nat*nat -> dep2.
+intros (p,q).
+exists p.
+exact q.
+Defined.
+ *)
+
+Definition lt_pq :dep2->dep2->Prop :=
+(lexprod nat (fun a => nat) Peano.lt (fun a:nat =>Peano.lt)).
+
+Definition le_pq (a b : dep2) : Prop :=
+  lt_pq a b \/ a = b.
+
+Lemma wf_lexprod : well_founded lt_pq.
+Proof.
+  unfold lt_pq; apply wf_lexprod.
+  apply lt_wf.
+  intro n.
+  apply lt_wf.
+Qed.
+
+(* Definition of lex lt. *)
+Definition llt : (nat*nat) -> (nat*nat) -> Prop :=
+  fun a b => lt_pq (mk2 a) (mk2 b).
+
+(* Definition of lex le. *)
+Definition lle : (nat*nat) -> (nat*nat) -> Prop :=
+  fun a b => le_pq (mk2 a) (mk2 b).
+
+Lemma wf_llt : well_founded llt.
+Proof.
+  unfold llt.
+  eapply wf_inverse_image.
+  apply wf_lexprod.
+Qed.
+
+Definition induction_llt := (well_founded_induction wf_llt).
