ind_lex_exp.v
@@ -1,0 +1,728 @@
+Require Import PeanoNat Lt.
+Require Import Lia.
+
+Theorem strong_induction_Prop:
+forall P : nat -> Prop,
+(forall n : nat, (forall k : nat, (k < n -> P k)) -> P n) ->
+forall n : nat, P n.
+Proof.
+  intros P Hind.
+  assert ((forall n k, k <= n -> P k) -> forall n, P n) as Hass.
+    intros HH n. eapply HH. eapply le_n.
+  eapply Hass. clear Hass.
+    induction n; intros k Hk. eapply PeanoNat.Nat.le_0_r in Hk.
+    subst. eapply Hind. intros k Hk. inversion Hk.
+
+    eapply Lt.le_lt_or_eq in Hk. destruct Hk.
+    eapply IHn. inversion H. apply le_n. subst. 
+    apply Le.le_Sn_le in H1.
+    assumption.
+    subst. apply Hind. firstorder.
+Qed.
+
+Theorem strong_induction:
+forall P : nat -> Type,
+(forall n : nat, (forall k : nat, (k < n -> P k)) -> P n) ->
+forall n : nat, P n.
+Proof.
+  intros P Hind.
+  assert ((forall n k, k <= n -> P k) -> forall n, P n) as Hass.
+    intros HH n. eapply HH. eapply le_n.
+  eapply Hass. clear Hass.
+  induction n; intros k Hk.
+    eapply PeanoNat.Nat.le_0_r in Hk.
+    subst. eapply Hind.
+    intros k Hk.
+    apply PeanoNat.Nat.nlt_0_r in Hk.
+    contradiction.
+    eapply Compare_dec.le_lt_eq_dec in Hk. 
+    destruct Hk.
+    eapply IHn. inversion l. apply le_n. subst. 
+    apply Le.le_Sn_le in H0.
+    assumption.
+    subst. apply Hind. firstorder.
+Qed.
+
+Locate well_founded.
+Print well_founded.
+
+Require Import Lia.
+
+SearchAbout le S lt.
+
+Require Import Wf.
+Require Import Relation_Operators.
+Require Import Lexicographic_Product.
+Require Import OrderedType.
+Require Import OrderedTypeEx.
+Require Import Wf_nat.
+
+
+Definition dep2 := sigT (A:=nat) (fun a => nat).
+
+Definition mk2 : nat*nat -> dep2.
+intros (p,q).
+exists p.
+exact q.
+Defined.
+
+Definition lt_pq :dep2->dep2->Prop :=
+(lexprod nat (fun a => nat) Peano.lt (fun a:nat =>Peano.lt)).
+
+Definition le_pq (a b : dep2) : Prop :=
+  lt_pq a b \/ a = b.
+
+Lemma wf_lexprod : well_founded lt_pq.
+unfold lt_pq;apply wf_lexprod.
+apply lt_wf.
+intro n.
+apply lt_wf.
+Qed.
+
+Definition lt_mine : (nat*nat) -> (nat*nat) -> Prop :=
+  fun a b => lt_pq (mk2 a) (mk2 b).
+
+Definition le_mine : (nat*nat) -> (nat*nat) -> Prop :=
+  fun a b => le_pq (mk2 a) (mk2 b).
+
+
+Require Import Inverse_Image.
+
+Lemma wf_lt_mine : well_founded lt_mine.
+Proof.
+  unfold lt_mine.
+  eapply wf_inverse_image.
+  apply wf_lexprod.
+Qed.
+
+SearchAbout "induction" well_founded.
+
+Definition induction_lt_mine := (well_founded_induction wf_lt_mine).
+
+(* Not good, because the last "P x" occurrence should be P (S x) for some kind of successor thing in this context - but which thing? Not appropriate for this context.
+Definition induction_le_mine :=
+  forall P : nat * nat -> Set,
+       (P (0,0)) -> 
+       (forall x : nat * nat, (forall y : nat * nat, le_mine y x -> P y) -> P x) ->
+       forall a : nat * nat, P a.
+*)
+
+Parameter P : (nat*nat) -> Set.
+
+SearchAbout "induction" nat.
+
+(*
+Lemma test2 : forall (n : nat), n = S n.
+Proof.
+  intros n.
+  induction (lt_wf n).
+
+  Print lt_wf.
+  Print 
+
+ *)
+
+Definition odd (n : nat) := exists k, n = 2*k + 1.
+Definition even (n : nat) := exists k, n = 2*k.
+
+Lemma test3 : forall (a : nat), odd a \/ even a.
+Proof.
+  intros a.
+  induction (lt_wf a) as [n _ IH].
+Admitted.
+
+
+Lemma test2 : forall (a : nat * nat), odd (fst a) \/ even (fst a).
+Proof.
+  induction a using induction_lt_mine.
+  destruct a as [n m]. simpl fst.
+  destruct n. right. unfold even. exists 0. auto.
+  destruct (H (n,m)). econstructor. firstorder.
+  simpl in H0. right. unfold odd in H0. unfold even.
+  destruct H0. exists (x+1). firstorder.
+  left.
+Admitted.
+
+Lemma test1 : forall a, P a -> (P a -> true = true).
+Proof.
+  intros a.
+  induction a using induction_lt_mine.
+Admitted.
+
+
+  
+
+
+(* Left it here 31/01/20.
+
+Use induction_lt_mine as induction principle.
+Write a test cases to make sure it'll work properly. 
+Start with something based off nats then something based of derivations.
+
+
+https://coq-club.inria.narkive.com/VWS50VZQ/adding-strong-induction-to-the-standard-library
+https://coq.inria.fr/refman/proof-engine/tactics.html#coq:tacv.induction-using
+https://coq.github.io/doc/master/stdlib/Coq.Structures.OrdersEx.html#PairOrderedType
+https://coq-club.inria.narkive.com/7Mts7wuN/how-to-show-lexicographic-product-of-three-well-founded-sets-is-well-founded
+https://coq.inria.fr/library/Coq.Arith.Wf_nat.html
+https://coq.github.io/doc/master/stdlib/Coq.Wellfounded.Lexicographic_Product.html
+https://coq.inria.fr/distrib/current/stdlib/Coq.Relations.Relation_Operators.html#lexprod
+https://stackoverflow.com/questions/42520130/lexicographical-comparison-of-tuples-of-nats
+https://coq.inria.fr/library/Coq.Init.Wf.html
+http://color.inria.fr/doc/CoLoR.Util.Pair.LexOrder.html
+https://coq.github.io/doc/master/stdlib/Coq.Arith.Compare.html
+https://coq.inria.fr/library/Coq.Structures.OrderedType.html
+https://coq.github.io/doc/master/stdlib/Coq.Structures.OrderedTypeEx.html
+https://coq.github.io/doc/master/stdlib/Coq.Structures.OrderedType.html
+
+*)
+  
+
+
+
+  unfold well_founded.
+  intros [n m].
+  simpl.
+
+
+
+Lemma lem : forall n m,
+    n < (S m) -> (n = m \/ n < m).
+Proof.
+  intros. lia.
+Qed.
+
+Theorem thm : well_founded lt.
+Proof.
+  unfold well_founded.
+  induction a. constructor.
+  intros y Hy. inversion Hy.
+  constructor. intros y Hy.
+  apply lem in Hy. destruct Hy.
+  subst. assumption.
+  eapply Acc_inv. apply IHa. assumption.
+Qed.
+
+Inductive mlex : (nat * nat) -> (nat * nat) -> Prop :=
+| mlexc1 a b n m : a < n -> mlex (a,b) (n,m)
+| mlexc2 a b n m : a = n -> b < m -> mlex (a,b) (n,m).
+Print Acc.
+
+Theorem thm2 : well_founded mlex.
+Proof.
+  unfold well_founded.
+  intros a. destruct a as [a b].
+  revert b.
+  induction a; intros b.
+  + induction b. constructor. intros [n m] H.
+    inversion H. subst. inversion H1. subst. inversion H5.
+    constructor. intros [n m] H. inversion H. subst.
+    inversion H1. subst.
+
+    inversion H5. subst. apply IHb.
+    subst. eapply Acc_inv. apply IHb.
+    constructor 2. auto. apply H1.
+
+  + induction b. econstructor.
+    intros [n m] H. inversion H. subst.
+    inversion H1. subst. eapply IHa.
+    subst. eapply Acc_inv. apply IHa.
+    constructor 1. apply H2.
+    subst. inversion H5.
+
+    inversion IHb as [H].
+    constructor. intros [n m] H2.
+    inversion H2. subst. inversion H1.
+    subst.  eapply IHa.
+    subst. specialize (IHa m).
+    eapply Acc_inv. apply IHa. constructor. apply H3.
+    subst. inversion H6. subst. apply IHb.
+    subst. eapply Acc_inv. apply IHb.
+    constructor 2. auto. apply H1.
+    Unshelve. auto.
+Qed.
+Print Assumptions thm2.
+
+Print well_founded_induction.
+Check (well_founded_induction thm2).
+
+Lemma attempt_to_use_ind : forall (P : (nat * nat) -> Set), forall n,
+      P n.
+Proof.
+  intros P n.
+  induction n using (well_founded_induction thm2).
+Abort.
+
+Check mlex_ind.
+
+Lemma mlex_induction_pre : forall (P : (nat * nat) -> Set),
+   forall a' b', P (0,0) ->
+    (forall a b, ( (forall n m, mlex (n,m) (a,b) -> P (n,m)) -> P (a,b))) ->
+    P (a',b').
+Proof.
+  intros P a b H1 H2.
+  remember (a,b) as c.
+  revert Heqc. revert b. revert a.
+  induction c using (well_founded_induction thm2).
+  intros a b Heqc.
+  subst. apply H2.
+  intros n m Hnm.
+  eapply H. 2 : reflexivity.
+  apply Hnm.
+Qed.
+
+Lemma mlex_induction_pre' : forall (P : (nat * nat) -> Set),
+   forall a' b', 
+    (forall a b, ( (forall n m, mlex (n,m) (a,b) -> P (n,m)) -> P (a,b))) ->
+    P (a',b').
+Proof.
+  intros P a b H2.
+  remember (a,b) as c.
+  revert Heqc. revert b. revert a.
+  induction c using (well_founded_induction thm2).
+  intros a b Heqc.
+  subst. apply H2.
+  intros n m Hnm.
+  eapply H. 2 : reflexivity.
+  apply Hnm.
+Qed.
+
+Lemma mlex_induction' : forall (P : (nat * nat) -> Set),
+    (forall a b, ( (forall n m, mlex (n,m) (a,b) -> P (n,m)) -> P (a,b))) ->
+   forall a b, P (a,b).
+Proof.  
+  intros. apply mlex_induction_pre'. auto. 
+Qed.
+
+Lemma lem1 : forall P,
+    (forall b, ( (forall a, a < b -> P a ) -> P b)) ->
+    P 0.
+Proof.
+  intros P H.
+  apply H.
+  intros a H2. unfold lt in H2.
+  Print le. Search le -max -min.
+  apply Le.le_n_0_eq in H2. discriminate.
+Qed.
+
+Lemma lem2 : forall P,
+    (forall b, ( (forall a, a <= b -> P a ) -> P b)) ->
+    P 0.
+Proof.
+  intros P H.
+  apply H.
+  intros a H2.
+  apply Le.le_n_0_eq in H2. subst.
+Abort.
+
+Print well_founded_induction.
+
+
+Lemma testing : forall (P : (nat * nat) -> Prop),
+     (forall a b, ( (forall n m, mlex (n,m) (a,b) -> P (n,m)) -> P (a,b))) ->
+    P (0,0).
+Proof.
+  intros .
+  apply H. intros.
+  inversion H0.
+  subst. inversion H2.
+  subst. inversion H6.
+Qed.
+
+Lemma nat_induction' : forall (P : nat -> Prop),
+    (forall m, (forall n, n < m -> P n) -> P m) ->
+   forall a, P a.
+Proof.  
+  intros. apply H.
+  intros n H2.
+  apply H. intros m Hm.
+  induction a. inversion H2.
+  inversion H2. subst. 
+Abort.
+     (*
+  induction  n; intros H2.
+  
+  apply mlex_induction_pre'. auto. 
+Qed.
+      *)
+     
+Print well_founded.
+
+Print lt.
+Locate lt.
+Search (?a <= ?a).
+
+Lemma mlex_induction : forall (P : (nat * nat) -> Set),
+   P (0,0) ->
+    (forall a b, ( (forall n m, mlex (n,m) (a,b) -> P (n,m)) -> P (a,b))) ->
+   forall a b, P (a,b).
+Proof.  
+  intros. apply mlex_induction_pre. auto. auto.
+Qed.
+
+
+Require Import Coq.Structures.OrdersEx.
+
+Module test_module2 := PairOrderedType Nat_as_DT Nat_as_DT.
+Module test_module := PairOrderedType Nat_as_OT Nat_as_OT.
+
+Print test_module.
+Print test_module2.
+
+(*
+Module
+test_module
+ : Sig
+     Definition t : Type.
+     Definition eq : Relation_Definitions.relation (nat * nat).
+     Definition eq_equiv : RelationClasses.Equivalence eq.
+     Definition eq_dec : forall x y : nat * nat, {eq x y} + {~ eq x y}.
+     Definition lt : Relation_Definitions.relation (nat * nat).
+     Parameter lt_strorder : RelationClasses.StrictOrder lt.
+     Parameter lt_compat :
+       Morphisms.Proper (Morphisms.respectful eq (Morphisms.respectful eq iff)) lt.
+     Definition compare : nat * nat -> nat * nat -> comparison.
+     Parameter compare_spec : forall x y : nat * nat, CompSpec eq lt x y (compare x y).
+   End
+:= (PairOrderedType Nat_as_OT Nat_as_OT)
+
+Module
+test_module2
+ : Sig
+     Definition t : Type.
+     Definition eq : Relation_Definitions.relation (nat * nat).
+     Definition eq_equiv : RelationClasses.Equivalence eq.
+     Definition eq_dec : forall x y : nat * nat, {eq x y} + {~ eq x y}.
+     Definition lt : Relation_Definitions.relation (nat * nat).
+     Parameter lt_strorder : RelationClasses.StrictOrder lt.
+     Parameter lt_compat :
+       Morphisms.Proper (Morphisms.respectful eq (Morphisms.respectful eq iff)) lt.
+     Definition compare : nat * nat -> nat * nat -> comparison.
+     Parameter compare_spec : forall x y : nat * nat, CompSpec eq lt x y (compare x y).
+   End
+:= (PairOrderedType Nat_as_DT Nat_as_DT)
+ *)
+Print lexprod.
+
+Import test_module.
+
+Print test_module.
+Locate lt.
+
+Infix "=" := eq (at level 70, no associativity) : test_module_scope.
+Infix "<" := lt (at level 70, no associativity) : test_module_scope.
+
+Open Scope test_module_scope.
+Locate "=".
+Print lt.
+SearchAbout well_founded.
+Print symprod.
+
+(*
+Lemma Acc_fst_0 : forall b, Acc lt (0,b).
+  induction b. econstructor.
+  intros y Hy.
+  inversion y as [a b].
+  inversion Hy. inversion H. inversion H.
+  inversion H1.
+  econstructor. intros [n m] H.
+  inversion H.
+  inversion H0.
+  inversion H0.
+  inversion H1. simpl in *.
+  subst. inverison H0.
+  inversion H0.  
+  
+ *)
+Definition lt_nat := Coq.Arith.PeanoNat.Nat.lt.
+Definition lt_nat2 := PeanoNat.Nat.compare.
+
+Lemma lt_fst_0 : forall a b m,
+    (a,b) < (0,m) -> a = 0.
+Proof.
+  intros a b m H.
+  inversion H as [H1 | H1].
+  inversion H1. inversion H1 as [H2 H3].
+  inversion H2. auto.
+Qed.
+
+Locate compare.
+Print lt_nat2.
+Print  PeanoNat.Nat.compare.
+
+
+
+
+Lemma lt_inv : forall a b n m,
+    (a,b) < (n,m) ->  ((a=n) /\ (b < m)%nat ) \/ (lt_nat a n).
+Proof.
+  firstorder.
+Qed.
+
+(*
+Lemma lt_inv : forall a b n m,
+    (a,b) < (n,m) ->  ((a=n) * ((lt_nat2 b m) = Lt)) + {lt_nat2 a n = Lt}.
+Proof.
+  intros a b n m H.
+  Print lt.
+  Print Relation_Definitions.relation.
+  inversion H.
+  case_eq (compare (a,b) (n,m)); intros H2.
+  *)
+
+
+Lemma not_lt_0 : forall a b, ~ (a,b) < (0,0).
+Proof.
+  intros a b H.
+  inversion H as [H1 | H1].
+  inversion H1. inversion H1 as [H2 H3].
+  inversion H3.
+Qed.
+
+Lemma lt_snd : forall a m n,
+    (m < n)%nat -> (a,m) < (a,n).
+Admitted.
+
+Lemma Acc_fst_0 : forall b, Acc lt (0,b).
+Proof.
+  induction b.
+  econstructor. intros [a b] H.
+  apply not_lt_0 in H. contradiction.
+
+  econstructor. intros [n m] H.
+  inversion IHb as [IH].
+  inversion H as [H1 | H1].
+  inversion H1. inversion H1 as [H2 H3].
+  inversion H2 as [H4]. simpl in H4. subst.
+  inversion H3 as [|H4 H5 H6]. subst.  assumption.
+  simpl in *. subst.
+  eapply IH.
+  apply lt_snd.
+  apply Lt.lt_S_n.
+  apply Lt.le_lt_n_Sm. assumption.
+Qed.
+
+(*
+Lemma lt_snd_0 : forall n, Acc lt (n,0).
+Proof.
+  induction n using (well_founded_induction _).
+  econstructor. intros [a b] H2.
+  apply lt_inv in H2. destruct H2 as [[H3 H4] | H3].
+  inversion H4.
+  
+  econstructor. intros [c d] Hc.
+  inversion 
+  apply not_lt_0 in H2. contradiction.
+  econstructor. intros [a b] H.
+  apply lt_inv in H. destruct H as [[H1 H2] | H1].
+  inversion H2.
+  
+
+
+  induction n using PeanoNat.Nat.lt_wf.  induction n.
+  econstructor. intros [a b] H.
+  apply not_lt_0 in H. contradiction.
+  econstructor. intros [a b] H.
+  apply lt_inv in H. destruct H as [[H1 H2] | H1].
+  inversion H2.
+  *)
+
+Lemma well_founded_lt : well_founded lt.
+Proof.
+  Search well_founded.
+  SearchAbout well_founded.
+  SearchAbout sum.
+SearchAbout relation_disjunction.
+  unfold lt.
+
+
+  unfold well_founded.
+  intros [n m].
+  revert m.
+  induction n using (well_founded_induction _); intros m.
+  econstructor. intros [a b] H2.
+  apply lt_inv in H2. destruct H2 as [[H3 H4] | H3].
+  subst.
+  assert ( (b < m)%nat -> Acc lt (x,m)   -> Acc lt (x,b)) as Hass.
+  admit. apply Hass. assumption.
+  apply H. 
+  apply le_n.
+
+  apply H.
+  admit.
+  Unshelve. 
+  apply H3.
+  Unshelve. unfold lt_nat.
+  firstorder.
+Qed.
+
+  SearchAbout well_founded PeanoNat.Nat.lt.
+  apply H. apply H2.
+  
+  induction n; econstructor.
+  + intros [a b] H.
+    apply lt_fst_0 in H.
+    subst. apply Acc_fst_0.
+  + intros [a b] H.
+    eapply lt_inv in H.
+    destruct H as [[H1 H2] | H1].
+    subst. econstructor.
+    intros [c d] H.
+    eapply lt_inv in H.
+    destruct H as [[H4 H5] | H4].
+    subst.
+    
+    inversion H as [H3| H3].
+    
+    inversion H as [[H11 H22] | H11].
+
+
+    
+
+Module test_module := PairOrderedType Nat_as_OT Nat_as_OT.
+
+Print test_module.
+
+Import test_module.
+
+Print test_module.
+
+Infix "=" := eq (at level 70, no associativity) : test_module_scope.
+Infix "<" := lt (at level 70, no associativity) : test_module_scope.
+
+Open Scope test_module_scope.
+Locate "=".
+Print lt.
+
+(*
+Lemma Acc_fst_0 : forall b, Acc lt (0,b).
+  induction b. econstructor.
+  intros y Hy.
+  inversion y as [a b].
+  inversion Hy. inversion H. inversion H.
+  inversion H1.
+  econstructor. intros [n m] H.
+  inversion H.
+  inversion H0.
+  inversion H0.
+  inversion H1. simpl in *.
+  subst. inverison H0.
+  inversion H0.  
+  
+ *)
+Definition lt_nat := Coq.Arith.PeanoNat.Nat.lt.
+
+Lemma lt_fst_0 : forall a b m,
+    (a,b) < (0,m) -> a = 0.
+Proof.
+  intros a b m H.
+  inversion H as [H1 | H1].
+  inversion H1. inversion H1 as [H2 H3].
+  inversion H2. auto.
+Qed.
+
+Lemma Acc_fst_0 : forall b, Acc lt (0,b).
+Proof.
+  induction b.
+  econstructor. intros [a b] H.
+Locate lt.
+  Lemma lt_inv : forall a b n m,
+    (a,b) < (n,m) -> {lt_nat a n} + {a=n * lt_nat b m}.
+  
+Admitted.
+  
+Lemma well_founded_le : well_founded lt.
+Proof.
+  unfold well_founded.
+  intros [n m].
+  induction n; econstructor.
+  + intros [a b] H.
+    apply lt_fst_0 in H.
+    subst. apply Acc_fst_0.
+    
+
+
+    
+    inversion H as [H1 | H2].
+    inversion H1.
+    inversion H2 as [H3 H4].
+    inversion H3. simpl in *.
+    subst. 
+    Print RelationPairs.RelProd.
+  induction a.
+
+
+Definition my_le := compare.
+
+Lemma test : forall (a : nat * nat), True.
+Import (PairOrderedType Nat_as_OT Nat_as_OT).
+
+Print Nat_as_OT.
+
+
+
+apply H. apply Hnm. 
+  induction n using (well_founded_induction thm2).
+
+  pose proof (well_founded_induction thm2 P) as H2. intros x IHx.
+  
+  pose proof (well_founded_induction thm2 P) as H2.
+  induction n using (well_founded_induction thm2).
+
+  destruct H1.
+
+
+  constructor. intros [n m] H.
+  inversion H; subst.
+  + inversion H1. subst. apply IHa.
+    subst. eapply Acc_inv. eapply IHa.
+    constructor. apply H2.
+  + eapply Acc_inv. eapply IHa. constructor 2. intros [c d] Hd.
+    
+    destruct H1.
+    ++ 
+  constructor. intros. inversion H.
+  + induction b. constructor.
+    intros [a b] H.
+    inversion H. subst. inversion H1.
+    subst. inversion H5.
+    constructor. intros [n m] H.
+    inversion H; subst.
+    inversion H1.
+    inversion H5. subst.  exact IHb.
+    subst. eapply Acc_inv.
+    exact IHb.
+    constructor 2. auto.
+    apply H1.
+  + induction b. constructor.
+    intros [n m] H. inversion H.
+    subst. inversion H1.
+    subst. eapply IHa.
+    subst.
+    eapply Acc_inv. eapply (IHa 0).
+    constructor. eapply H2.
+    subst. inversion H5.
+    
+
+    destruct H2.
+    destruct H1.
+    eapply Acc_inv. eapply IHa.
+    inversion H. subst.
+
+    
+    eapply Acc_inv. exact IHb.
+    
+    eapply (@Acc_inv _ mlex) in IHb.
+    exact IHb.
+    
+    constructor. intros 
+    eapply Acc_inv in IHb.
+    eexact IHb.
+
+    constructor. intros [n m] H.
+    inversion H. subst.
+    inversion H1. subst. 
+    inversion H5. subst.
+    constructor. intros [a b] Hb.
+    inversion Hb. subst. inversion H1. subst.
+  
