merge.v
@@ -1,0 +1,210 @@
+Require Import List.
+Export ListNotations.
+
+Require Import lntT List_lemmasT.
+Require Import existsT.
+Require Import contractedT.
+Require Import Coq.Classes.CRelationClasses.
+Require Import structural_equivalence.
+
+Ltac clear_useless :=
+  repeat match goal with
+         | [H : ?a = ?a |- _] => clear H
+         | [H : [?a] = [?a] |- _] => clear H
+         | [H : ?a :: ?b = ?a :: ?b |- _] => clear H
+         | [H1 : ?a, H2 : ?a |- _] => clear H2
+         end.
+
+Ltac inv_singleton :=
+    repeat ( match goal with
+       | [ H : ?a :: [] = ?c :: ?d |- _ ] => inversion H; subst
+       | [ H : ?a :: ?b = ?c :: [] |- _ ] => inversion H; subst
+       | [ H : ?a :: ?b = ?c :: ?d |- _ ] => inversion H; subst
+       | [ H : ((?a,?b) = ?c) |- _ ] => inversion H; subst
+       | [ H : ?c = (?a,?b) |- _ ] => inversion H; subst
+             end; clear_useless).
+
+Inductive merge {V : Set} :  (list (rel (list (PropF V)) * dir)) ->  (list (rel (list (PropF V)) * dir)) ->  (list (rel (list (PropF V)) * dir)) -> Type :=
+| merge_nilL ns1 ns2 ns3 : ns1 = [] -> ns3 = ns2 -> merge ns1 ns2 ns3
+| merge_nilR ns1 ns2 ns3 : ns2 = [] -> ns3 = ns1 -> merge ns1 ns2 ns3
+| merge_step Γ Δ Σ Π d ns1 ns2 ns3 ns4 ns5 ns6 seq1 seq2 seq3 :
+    seq1 = (Γ,Δ,d) -> seq2 = (Σ,Π,d) -> seq3 = (Γ++Σ,Δ++Π,d) ->
+    merge ns1 ns2 ns3 ->
+    ns4 = seq1 :: ns1 -> ns5 = seq2 :: ns2 -> ns6 = seq3 :: ns3 ->
+    merge ns4 ns5 ns6.
+
+Lemma merge_existence {V : Set} : forall n1 n2,
+      struct_equiv_weak n1 n2 ->
+      existsT2 n3, @merge V n1 n2 n3.
+Proof.
+  induction n1; intros n2  Hequiv.
+  inversion Hequiv. subst. inversion H0; subst.
+  simpl in *. subst. exists nil. econstructor; reflexivity.
+  discriminate.
+  subst. inversion H0. subst. simpl in *.
+  exists ns3. econstructor 1; reflexivity.
+  discriminate.
+
+  destruct n2. exists (a :: n1). econstructor 2; reflexivity.
+  destruct a as [ [Γ1 Δ1] d1].
+  destruct p as [ [Γ2 Δ2] d2].
+  pose proof (struct_equiv_weak_d _ _ _ _ _ _ Hequiv). subst.
+  eapply struct_equiv_weak_cons in Hequiv.
+  eapply IHn1 in Hequiv. destruct Hequiv as [n3 Hn3].
+  exists ((Γ1 ++ Γ2, Δ1 ++ Δ2, d2) :: n3).
+  econstructor 3; try reflexivity. assumption.
+Qed.
+
+Lemma merge_consL : forall {V : Set} l l2 a b c,
+    @merge V (a :: l) [b] (c :: l2) ->
+    l = l2.
+Proof.
+  intros until 0; intros Hm.
+  inversion Hm; try discriminate;
+    inv_singleton; try reflexivity.
+  inversion X; try discriminate;
+  subst; reflexivity.
+Qed.  
+
+
+Lemma merge_consR : forall {V : Set} l l2 a b c,
+    @merge V [b] (a :: l) (c :: l2) ->
+    l = l2.
+Proof.
+  intros until 0; intros Hm.
+  inversion Hm; try discriminate;
+    inv_singleton; try reflexivity.
+  inversion X; try discriminate;
+  subst; reflexivity.
+Qed.  
+
+Lemma merge_unique {V : Set} : forall n1 n2 n3 n4,
+    struct_equiv_weak n1 n2 ->
+    merge n1 n2 n3 -> @merge V n1 n2 n4 -> n3 = n4.
+Proof.
+  induction n1; intros n2 n3 n4 Hs Hm1 Hm2.
+  inversion Hm1; subst; inversion Hm2; subst;
+    try reflexivity; try discriminate.
+
+  inversion Hm1; inversion Hm2; subst; try discriminate; try reflexivity;
+    inv_singleton; try reflexivity.
+
+  all : try solve [inversion X; subst; try reflexivity; try discriminate].
+
+  eapply IHn1 in X; [ | | exact X0].
+  subst. reflexivity.
+  eapply struct_equiv_weak_cons. exact Hs.
+Qed.
+
+Lemma merge_struct_equiv_weak : forall {V : Set} G1 G2 G3,
+  merge G1 G2 G3 ->
+  @struct_equiv_weak V G1 G2.
+Proof.
+  induction G1; intros G2 G3 H.
+  + inversion H; try discriminate.
+    econstructor 2. erewrite app_nil_l. reflexivity. econstructor.
+    econstructor 2. erewrite app_nil_l. reflexivity. econstructor.    
+  + inversion H; try discriminate.
+  -{ inversion H0.
+     subst. econstructor 1.
+     erewrite app_nil_l. reflexivity.    
+     econstructor.
+   }
+  -{ subst. inv_singleton.
+     eapply struct_equiv_weak_cons_rev.
+     eapply IHG1. eassumption.
+   }
+Qed.
+
+Lemma merge_nil : forall {V : Set} ns,
+    @merge V [] [] ns -> ns = [].
+Proof.
+  induction ns; intros Hm. auto.
+  inversion Hm; try discriminate.
+Qed.
+
+Lemma merge_ex_str : forall {V : Set} G1 G2,
+    struct_equiv_str G1 G2 -> existsT2 G3, @merge V G1 G2 G3.
+Proof.
+  induction G1; intros G2 Hs.
+  inversion Hs. exists []. constructor; reflexivity.
+  discriminate.
+  inversion Hs; try discriminate.
+  inv_singleton. eapply IHG1 in H1.
+  destruct H1 as [G3 H1].
+  eexists ( (Γ1 ++ Γ2, Δ1 ++ Δ2, d) :: G3).
+  econstructor 3; try reflexivity. assumption.
+Qed.
+
+Lemma merge_appLR : forall {V : Set} G1 G2 G3 G,
+    merge G1 G2 G3 ->
+    length G1 = length G2 ->
+    @merge V (G1 ++ G) G2 (G3 ++ G).
+Proof.
+  induction G1; intros until 0; intros Hm Hl.
+  +{ destruct G2. inversion Hm; try discriminate.
+     subst. simpl. econstructor 2; reflexivity.
+     subst. simpl. econstructor 2; reflexivity.
+     discriminate.
+   }
+  +{ destruct G2. discriminate.
+     simpl in Hl. inversion Hl as [Hl'].
+     simpl. destruct G3. inversion Hm; discriminate.
+
+     simpl. inversion Hm; try discriminate.
+     subst. inv_singleton.
+     eapply IHG1 in X.
+     econstructor 3; try reflexivity.
+     eassumption. assumption.
+   }
+Qed.
+
+Lemma merge_appRR : forall {V : Set} G1 G2 G3 G,
+    merge G1 G2 G3 ->
+    length G1 = length G2 ->
+    @merge V (G1) (G2 ++ G) (G3 ++ G).
+Proof.
+  induction G1; intros until 0; intros Hm Hl.
+  +{ destruct G2. inversion Hm; try discriminate.
+     subst. simpl. econstructor 1; reflexivity.
+     subst. simpl. econstructor 1; reflexivity.
+     discriminate.
+   }
+  +{ destruct G2. discriminate.
+     simpl in Hl. inversion Hl as [Hl'].
+     simpl. destruct G3. inversion Hm; discriminate.
+
+     simpl. inversion Hm; try discriminate.
+     subst. inv_singleton.
+     eapply IHG1 in X.
+     econstructor 3; try reflexivity.
+     eassumption. assumption.
+   }
+Qed.
+
+Lemma merge_ex : forall {V : Set} G1 G2,
+    struct_equiv_weak G1 G2 -> existsT2 G3, @merge V G1 G2 G3.
+Proof.
+  intros until 0; intros Hs.
+  inversion Hs; subst;
+  pose proof H0 as H0';
+  eapply struct_equiv_str_length in H0';
+  eapply merge_ex_str in H0;
+  destruct H0 as [G3 H0];
+  exists (G3 ++ ns3).
+
+  eapply merge_appLR; assumption.
+  eapply merge_appRR; assumption.
+Qed.
+
+Lemma merge_contracted_nseq : forall {V : Set} G H,
+  @merge V G G H ->
+  contracted_nseq H G.
+Proof.
+  induction G; intros H Hm.
+  eapply merge_nil in Hm. subst. econstructor.
+  inversion Hm; try discriminate.
+  inv_singleton.
+  econstructor. eapply contracted_seq_double.
+  apply IHG. assumption.
+Qed.
