structural_equivalence.v
@@ -1,0 +1,189 @@
+Require Import List.
+Export ListNotations.
+
+Require Import lntT List_lemmasT.
+Require Import existsT.
+Require Import contractedT.
+Require Import Coq.Classes.CRelationClasses.
+
+Ltac clear_useless :=
+  repeat match goal with
+         | [H : ?a = ?a |- _] => clear H
+         | [H : [?a] = [?a] |- _] => clear H
+         | [H : ?a :: ?b = ?a :: ?b |- _] => clear H
+         | [H1 : ?a, H2 : ?a |- _] => clear H2
+         end.
+
+Ltac inversion_cons :=
+  repeat match goal with
+         | [ H : ?a :: ?l1 = ?b :: ?l2 |- _] => inversion H; subst; clear_useless
+         end.
+
+(* Use this one to help with full structural equivalence definition. *)
+Inductive struct_equiv_str {V : Set} : (list (rel (list (PropF V)) * dir)) -> (list (rel (list (PropF V)) * dir)) -> Type :=
+| se_nil2 : struct_equiv_str [] []
+| se_step2 Γ1 Δ1 d Γ2 Δ2 ns1 ns2 ns3 ns4 :
+    ns3 = ((Γ1, Δ1, d) :: ns1) ->
+    ns4 = ((Γ2, Δ2, d) :: ns2) ->
+    struct_equiv_str ns1 ns2 ->
+    struct_equiv_str ns3 ns4.
+
+(* Use this one for structural equivalence. *)
+Inductive struct_equiv_weak {V : Set} : (list (rel (list (PropF V)) * dir)) -> (list (rel (list (PropF V)) * dir)) -> Type :=
+| se_wk2_extL ns1 ns2 ns3 ns4 :
+    ns4 = (ns1 ++ ns3) -> struct_equiv_str ns1 ns2 -> struct_equiv_weak ns4 ns2
+| se_wk2_extR ns1 ns2 ns3 ns4 :
+    ns4 = (ns2 ++ ns3) -> struct_equiv_str ns1 ns2 -> struct_equiv_weak ns1 ns4.
+
+Inductive struct_equiv {V : Set} n1 n2 : Type :=
+| se : @struct_equiv_weak V n1 n2 -> struct_equiv n1 n2.
+
+Lemma struct_equiv_str_weak : forall {V : Set} G1 G2,
+   @struct_equiv_str V G1 G2 -> @struct_equiv_weak V G1 G2.
+Proof.
+  intros V G1 G2 H.
+  eapply se_wk2_extL in H. 2 : reflexivity.
+  erewrite app_nil_r in H.  exact H.
+Qed.
+
+Lemma struct_equiv_str_length : forall {V : Set} G1 G2,
+    @struct_equiv_str V G1 G2 -> length G1 = length G2.
+Proof.
+  induction G1; intros H2 H; destruct H2;
+    subst; (reflexivity || inversion H).
+  discriminate. discriminate. 
+  subst. simpl. erewrite IHG1. reflexivity.
+  inversion H1. inversion H0. subst.
+  assumption.
+Qed.
+
+Lemma struct_equiv_weak_str : forall {V : Set} G1 G2,
+    @struct_equiv_weak V G1 G2 -> length G1 = length G2 ->
+    @struct_equiv_str V G1 G2.
+Proof.
+  intros V G1 G2 H1 H2.
+  inversion H1; subst;
+    rewrite app_length in H2.
+  inversion H0; subst. simpl in *.
+  apply length_zero_iff_nil in H2. subst.
+  constructor.
+  simpl; pose proof H4 as H4';
+  eapply struct_equiv_str_length in H4;
+  simpl in H2; rewrite H4 in H2;
+  destruct ns3; simpl in *; [
+  rewrite app_nil_r;  econstructor; try reflexivity; try assumption |
+  firstorder ].
+
+  inversion H0; subst. simpl in *.
+  symmetry in H2.
+  apply length_zero_iff_nil in H2. subst.
+  constructor.
+  simpl; pose proof H4 as H4';
+  eapply struct_equiv_str_length in H4;
+  simpl in H2; rewrite H4 in H2;
+  destruct ns3; simpl in *; [
+  rewrite app_nil_r;  econstructor; try reflexivity; try assumption |
+  firstorder ].
+Qed.
+
+Lemma struct_equiv_weak_cons : forall {V : Set} l1 l2 a1 a2,
+    struct_equiv_weak (a1::l1) (a2::l2) ->
+    @struct_equiv_weak V l1 l2.
+Proof.
+  intros V l1 l2 a1 a2 H3.
+  inversion H3 as [l3 H4 l4 H5 H6 H7 | H4 l3 l4 H5 H6 H7]; subst.
+  destruct l3 as [| a ns1];
+    inversion H7; try discriminate; subst.
+  simpl in *. unfold rel in *.
+  inversion_cons.
+  econstructor. reflexivity. assumption.
+
+  destruct l3 as [| a ns1];
+    inversion H7; try discriminate; subst.
+  simpl in *. unfold rel in *.
+  inversion_cons.
+  econstructor 2. reflexivity. assumption.
+Qed.
+
+Lemma struct_equiv_weak_cons_rev : forall {V : Set} l1 l2 a1 a2 b1 b2 d,
+    @struct_equiv_weak V l1 l2 ->
+    struct_equiv_weak ((a1,b1,d)::l1) ((a2,b2,d)::l2).
+Proof.
+  intros V l1 l2 a1 a2 b1 b2 d H3.
+  inversion H3; subst.
+  econstructor.
+  rewrite cons_singleton. rewrite app_assoc.
+  reflexivity.
+  econstructor 2; try reflexivity. assumption.
+
+  econstructor 2.  rewrite cons_singleton. rewrite app_assoc.
+  reflexivity.
+  econstructor 2; try reflexivity. assumption.
+Qed.
+
+Ltac struct_equiv_str_nil :=
+  match goal with
+  | [H : struct_equiv_str [] ?n |- _] => inversion H; discriminate
+  | [H : struct_equiv_str ?n [] |- _] => inversion H; discriminate
+  end.
+
+Ltac struct_equiv_str_cons :=
+  match goal with
+  | [H : struct_equiv_str (?a :: ?la) (?b :: ?lb) |- _] => inversion H; subst
+  end.
+
+Lemma struct_equiv_weak_d : forall {V : Set} ns1 ns2 seq1 seq2 d1 d2,
+    @struct_equiv_weak V ((seq1,d1)::ns1) ((seq2,d2)::ns2) ->
+    d1 = d2.
+Proof.
+  intros until 0; intros H3.
+  inversion H3 as [l3 H4 l4 H5 H6 H7 | H4 l3 l4 H5 H6 H7]; subst. 
+  destruct l3. simpl in *.
+  struct_equiv_str_nil.
+  simpl in *.
+  inversion_cons.
+  struct_equiv_str_cons. 
+  unfold rel in *. inversion_cons.
+  reflexivity.
+  
+  destruct l3. simpl in *.
+  struct_equiv_str_nil.
+  simpl in *.
+  inversion_cons.
+  struct_equiv_str_cons. 
+  unfold rel in *. inversion_cons.
+  reflexivity.
+Qed.  
+
+Lemma struct_equiv_str_weak_equiv : forall {V : Set} G1 G2,
+    iffT (@struct_equiv_str V G1 G2)
+         (struct_equiv_weak G1 G2 * (length G1 = length G2)).
+Proof.
+  intros.
+  split; intros HH. split. apply struct_equiv_str_weak.
+  assumption. apply struct_equiv_str_length. assumption.
+  apply struct_equiv_weak_str; apply HH.
+Qed.
+
+Lemma struct_equiv_weak_nil : forall (V : Set),
+    @struct_equiv_weak V nil nil.
+Proof.
+  econstructor. erewrite app_nil_r.
+  reflexivity. econstructor.
+Qed.
+  
+Lemma struct_equiv_str_refl : forall {V : Set} G, @struct_equiv_str V G G.
+Proof.
+  induction G as [|a G IHG]. constructor.
+  destruct a as [ [Γ Δ] d].
+  econstructor 2. reflexivity.
+  reflexivity. assumption.
+Qed.
+
+Lemma struct_equiv_weak_refl : forall {V : Set} G,
+    @struct_equiv_weak V G G.
+Proof.
+  intros V G. econstructor.
+  erewrite app_nil_r. reflexivity.
+  apply struct_equiv_str_refl.
+Qed.
